theories/interop/wrapper_wp_simulation.v
@@ -11,7 +11,7 @@ From melocoton Require Import big_sepM_limited.
 From iris.proofmode Require Import proofmode.
 From melocoton.c_toy_lang Require Import lang melocoton.lang_instantiation melocoton.primitive_laws.
 From melocoton.ml_toy_lang Require Import lang melocoton.lang_instantiation melocoton.primitive_laws.
-From melocoton.interop Require Import linking_wp basics wrapper_wp wrapper_wp_block_sim.
+From melocoton.interop Require Import linking_wp basics wrapper_wp wrapper_wp_block_sim wrapper_wp_utils wrapper_wp_ext_call_laws.
 Import Wrap.
 
 Section Simulation.
@@ -21,6 +21,9 @@ Context {Σ : gFunctors}.
 Context `{!heapGS_ML Σ, !heapGS_C Σ}.
 Context `{!invGS_gen hlc Σ}.
 Context `{!wrapperGS Σ}.
+
+Context (p : language.prog C_lang).
+Context (Hforbid : Forall (fun k => p !! k = None) forbidden_function_names).
 
 Notation MLval := ML_lang.val.
 Notation Cval := C_lang.val.
@@ -32,95 +35,9 @@ Import mlanguage.
 Notation mkPeC p T := ({| penv_prog := p; penv_proto := T |} : prog_environ _ Σ).
 Notation mkPeW p T := ({| weakestpre.penv_prog := p; weakestpre.penv_proto := T |} : weakestpre.prog_environ wrap_lang Σ).
 
-
-Definition WP_ext_call_spec : string -d> list Cval -d> (Cval -d> iPropO Σ) -d> iPropO Σ := λ n vl wp,
-  ⌜False⌝%I.
-
-Definition forbidden_function_names : list string := ["alloc"; "registerroot"; "unregisterroot"; "modify"; "readfield"; "int2val"; "val2int"].
-
 Notation wrap_return := (fun Φ (a:Cval) => (∃ θ' l v, GC θ' ∗ Φ v ∗ ⌜repr_lval θ' l a⌝ ∗ block_sim v l)%I).
 
-Lemma repr_roots_dom θ a b : repr_roots θ a b -> dom a = dom b.
-Proof.
-  induction 1.
-  + by do 2 rewrite dom_empty_L.
-  + by do 2 rewrite dom_insert_L; rewrite IHrepr_roots.
-Qed.
-
-(* We can decompose mem, the C heap, into a privmem, which is everything but the roots, and a memr, which are just the rooted cells *)
-Lemma make_repr θ roots_m mem : 
-    roots_are_live θ roots_m
- -> map_Forall (λ k v, ∃ w , mem !! k = Some (Storing w) ∧ repr_lval θ v w) roots_m
- -> ∃ privmem, repr θ roots_m privmem mem.
-Proof.
-  revert mem.
-  induction roots_m as [|l a roots_m Hin IH] using map_ind; intros mem Hlive Hforall.
-  + exists mem, ∅. split_and!.
-    * econstructor.
-    * eapply map_disjoint_empty_r.
-    * by rewrite map_empty_union.
-  + apply map_Forall_insert_1_1 in Hforall as Hforall2.
-    destruct Hforall2 as (w & Hw & Hrep).
-    specialize (IH (delete l mem)).
-    destruct IH as (privmem & memr & IH & Hdisj & Hunion).
-    1: intros l' g Hg; eapply Hlive; rewrite lookup_insert_ne; first done; intros ->; rewrite Hg in Hin; congruence.
-    1: apply map_Forall_lookup; intros i x Hinix;
-       eapply map_Forall_lookup_1 in Hforall.
-    1: destruct Hforall as (w' & H1 & H2); exists w'; repeat split; try done.
-    1: rewrite lookup_delete_ne; first done.
-    2: rewrite lookup_insert_ne; first done.
-    1-2: intros ->; rewrite Hin in Hinix; congruence.
-    assert (memr !! l = None) as HNone1.
-    1: apply not_elem_of_dom; erewrite <- repr_roots_dom; last done; by eapply not_elem_of_dom.
-    assert (privmem !! l = None) as Hnone2.
-    rewrite <- (lookup_union_r memr privmem); try done; rewrite <- Hunion; by apply lookup_delete.
-    eexists privmem, (<[l:=Storing w]> memr). split_and!.
-    * econstructor; try done; by eapply not_elem_of_dom.
-    * by apply map_disjoint_insert_r.
-    * erewrite <- insert_union_l. rewrite <- Hunion. rewrite insert_delete_insert.
-      apply map_eq_iff. intros i. destruct (decide (i = l)) as [-> |]; (try by rewrite lookup_insert); by rewrite lookup_insert_ne.
-Qed.
-
-Lemma repr_lval_inj θ v w w' : repr_lval θ v w -> repr_lval θ v w' -> w = w'.
-Proof.
-  induction 1; inversion 1.
-  + done.
-  + rewrite H in H3. injection H3; intros ->; done.
-Qed.
-
-Lemma set_to_none θ mem roots_m privmem :
-    repr θ roots_m privmem mem
- -> gen_heap_interp mem
- -∗ ([∗ map] a0↦v0 ∈ roots_m, ∃ w, a0 ↦C{DfracOwn 1} w ∗ ⌜repr_lval θ v0 w⌝)
-==∗ (gen_heap_interp (privmem ∪ ((λ _ : lval, None) <$> roots_m))
-    ∗[∗ set] a0 ∈ dom roots_m, a0 O↦ None).
-Proof.
-  intros (mm & Hrepr1 & Hrepr2 & Hrepr3).
-  induction Hrepr1 in Hrepr2,Hrepr3,mem,privmem|-*.
-  + iIntros "Hheap Hmap !>".
-    rewrite fmap_empty. rewrite dom_empty_L. rewrite map_union_empty.
-    rewrite map_empty_union in Hrepr3. subst mem. iFrame.
-    iApply big_sepS_empty. done.
-  + eapply not_elem_of_dom in H0,H1. iIntros "Hheap Hmap".
-    iPoseProof (big_sepM_insert) as "(Hb1 & _)"; first apply H0.
-    iPoseProof ("Hb1" with "Hmap") as "((%w' & Hw & %Hrepr4) & Hmap)".
-    pose proof (repr_lval_inj _ _ _ _ Hrepr4 H) as Heq; subst w'.
-    iMod (gen_heap_update with "Hheap Hw") as "(Hheap & Hw)".
-    specialize (IHHrepr1 (<[a:=None]> mem) (<[a:=None]> privmem)).
-    iMod (IHHrepr1 with "Hheap Hmap") as "(Hheap & Hmap)".
-    * eapply map_disjoint_insert_l_2; first done.
-      erewrite <- (delete_insert mem0); last done.
-      by eapply map_disjoint_delete_r.
-    * subst mem. erewrite <- insert_union_l.
-      rewrite insert_insert. by rewrite insert_union_r.
-    * iModIntro. iSplitL "Hheap".
-      - erewrite <- insert_union_l. rewrite insert_union_r.
-        2: eapply map_disjoint_Some_r; try done; by rewrite lookup_insert.
-        rewrite fmap_insert. iFrame.
-      - rewrite dom_insert_L. iApply big_sepS_insert; first by eapply not_elem_of_dom. iFrame.
-Qed.
-
-Lemma wp_to_val E p T a Φ: 
+Lemma wp_to_val E T a Φ: 
     wrap_return Φ a (* Basically, a WP (Val a) {{a, wrap_return a}} *)
  -∗ not_at_boundary
  -∗ WP (ExprC (C_lang.Val a)) @ (mkPeW (p : prog wrap_lang) T); E {{ v, Φ v ∗ at_boundary _}}.
@@ -158,19 +75,9 @@ Proof.
   1: by assert ((1 / 4 + 1 / 4 = 1 / 2)%Qp) as -> by compute_done.
   destruct (make_repr (θC ρc) roots_m mem) as [privmem Hpriv]; try done.
   iMod (ghost_var_update_halves with "HAGCθ HAθ") as "(HAGCθ & HAθ)".
-(*
-  iAssert (⌜gmap_inj χvirt⌝)%I as "%Hinj".
-  1: { iPoseProof (gset_bij_own_valid with "HAχbij") as "%Hbij". iPureIntro.
-       destruct Hbij as (_ & Hbij). intros l1 l2 vv Hl1 Hl2.
-       eapply gset_bijective_eq_iff. 1: apply Hbij.
-       1-2: eapply elem_of_map_to_set_pair. all: done. } *)
   iMod (set_to_none with "HσC Hrootspto") as "(HσC & Hrootspto)".
   1: done.
-(*
-  assert (val_safe_on_heap σMLvirt v) as Hsafe.
-  1: { eapply is_val_is_safe_on_heap; last done. destruct Hstore_blocks; set_solver. }
-  iMod (val_safe_to_ghost_state with "[] HAσdom") as "(HAσdom & #Hsafe)"; first done.
-*)
+
   do 3 iModIntro. do 2 iExists _.  iSplit.
   1: iPureIntro; eapply (H4 σMLvirt l v ζfreeze ζσ χvirt ζrest roots_m privmem).
   all: try done.
@@ -181,26 +88,14 @@ Proof.
   cbn. iSplitL "HAσMLv HAnMLv HAσdom".
   1: iExists nMLv; iFrame.
   unfold private_state_interp, ML_state_interp, GC_token_remnant, named; cbn.
-  iFrame "HArootss".
-  iFrame "HArootsm".
-  iFrame "HAGCθ".
-  iFrame "HAζrest".
-  iSplitL "HσC HnC"; first (iExists nCv; iFrame).
-  iFrame "HAχvirt".
-  iFrame "HAχNone".
-  iFrame "Hbound".
-  iFrame "HAθ".
+  iFrame. iSplitL "HnC"; first by iExists _.
   rewrite <- Hagree2.
-  iFrame "Hrootspto".
   iFrame "HAroots".
   iPureIntro; split_and!.
   1: destruct Hχvirt as (_ & HHH); apply HHH.
   1: apply Hother_blocks.
   1: destruct Hpriv as (mem_r & ->%repr_roots_dom & Hpriv2 & Hpriv3); by apply map_disjoint_dom.
 Qed.
-
-Context (p : language.prog C_lang).
-Context (Hforbid : Forall (fun k => p !! k = None) forbidden_function_names).
 
 Lemma wp_simulates E T ec Φ: 
     not_at_boundary
@@ -229,7 +124,17 @@ Proof.
     iFrame.
     iSplitL "HAnMLv"; first by iExists nMLv.
     iPureIntro. split_and!; done.
-  + cbn. iExFalso. iApply "HT". (* TODO: add more calls here *)
+  + iPoseProof (wp_ext_call_collect_all with "[] Hnb HT [Hr]") as "Hwp"; first done.
+    1: iIntros "!> %r HΞ Hnb"; iApply ("IH" with "Hnb");
+       by iApply "Hr".
+    rewrite weakestpre.wp_unfold. rewrite /weakestpre.wp_pre.
+    iApply ("Hwp" $! (CState ρc mem)).
+    iSplitL "Hσ". 1: by iExists _.
+    unfold C_state_interp, named.
+    iExists ζfreeze, ζσ, ζrest, χvirt, σMLvirt.
+    iFrame.
+    iSplitL "HAnMLv"; first by iExists nMLv.
+    iPureIntro. split_and!; done.
   + cbn in Hred. iModIntro. iRight. iRight. iSplit.
     * iPureIntro. exists (fun _ => True). eapply head_prim_step.
       destruct Hred as (e' & σ' & Hprim). econstructor; last done. cbn. eapply Hprim.
@@ -257,562 +162,8 @@ Proof.
       iPureIntro; split_and!; done.
 Qed.
 
-Definition lookup_reversed (χ : lloc_map) ℓ := {γ | χ !! γ = Some (LlocPublic ℓ)}.
-
-Definition find_in_χ (χ:lloc_map) ℓ : sum (lookup_reversed χ ℓ) (lookup_reversed χ ℓ -> False).
-Proof.
-  pose (map_to_set (fun γ ll => match ll with LlocPrivate => None | LlocPublic ℓ' => if decide (ℓ' = ℓ) then Some γ else None end) χ : gset _) as Hset.
-  epose (filter (fun k => is_Some (k)) Hset) as Hset2.
-  destruct (elements Hset2) as [|[γ|] ?] eqn:Heq.
-  - right. intros (γ & Hγ).
-    apply elements_empty_inv in Heq. apply gset_leibniz in Heq.
-    eapply filter_empty_not_elem_of_L. 2: apply Heq. 1: apply _.
-    2: eapply elem_of_map_to_set.
-    2: exists γ, (LlocPublic ℓ); split; done.
-    rewrite decide_True; done. Unshelve. all: apply _.
-  - left. exists γ.
-    assert (Some γ ∈ Hset2).
-    1: eapply elem_of_elements; rewrite Heq; left.
-    eapply elem_of_filter in H. destruct H as [_ H].
-    eapply elem_of_map_to_set in H.
-    destruct H as (i & ll & H1 & H2).
-    destruct ll; try congruence.
-    destruct decide; try congruence.
-  - exfalso. assert (None ∈ Hset2).
-    + eapply elem_of_elements. rewrite Heq. left.
-    + apply elem_of_filter in H. destruct H as [[? Hc]?]. congruence.
-Defined.
-
-Lemma ensure_in_χ_pub χ ℓ : lloc_map_inj χ → exists χ' γ, lloc_map_mono χ χ' ∧ χ' !! γ = Some (LlocPublic ℓ) ∧ ∀ γ' r, γ' ≠ γ → χ' !! γ' = r → χ !! γ' = r.
-Proof.
-  intros Hinj.
-  destruct (find_in_χ χ ℓ) as [[γ Hgam]|Hnot].
-  1: exists χ, γ; done.
-  eexists (<[fresh (dom χ) := LlocPublic ℓ]> χ), _.
-  erewrite lookup_insert; split_and!. 2: done.
-  2: intros γ' r Hne H1; by rewrite lookup_insert_ne in H1.
-  split.
-  1: eapply insert_subseteq, not_elem_of_dom, is_fresh.
-  intros γ1 γ2 ℓ' [[? ?]|[? ?]]%lookup_insert_Some [[? ?]|[? ?]]%lookup_insert_Some; subst.
-  1: done.
-  3: by eapply Hinj.
-  all: exfalso; eapply Hnot; eexists _; erewrite H0, H2; done.
-Qed.
-
-Definition extended_to (χold : lloc_map) (ζ : lstore) (χnew : lloc_map) :=
-  lloc_map_mono χold χnew ∧ dom χold ## dom ζ ∧ is_private_blocks χnew ζ.
-
-Lemma extended_to_inj χ1 ζ χ2 : extended_to χ1 ζ χ2 → lloc_map_inj χ2.
-Proof.
-  intros (H&_); apply H.
-Qed.
-
-Lemma extended_to_dom_subset χ1 ζ χ2 : extended_to χ1 ζ χ2 → dom ζ ⊆ dom χ2.
-Proof.
-  intros (H1&H2&H3).
-  eapply elem_of_subseteq. intros γ Hx; eapply elem_of_dom_2. by apply H3.
-Qed.
-
-Definition allocate_in_χ_priv (χold : lloc_map) v : lloc_map_inj χold → exists χnew γ, extended_to χold {[γ := v]} χnew.
-Proof.
-  intros Hinj.
-  eexists (<[fresh (dom χold) := LlocPrivate]> χold), (fresh (dom χold)).
-  unfold extended_to; split_and!; first split.
-  - eapply insert_subseteq, not_elem_of_dom, is_fresh.
-  - intros γ1 γ2 ℓ' [[? ?]|[? ?]]%lookup_insert_Some [[? ?]|[? ?]]%lookup_insert_Some; subst; try congruence.
-    by eapply Hinj.
-  - rewrite dom_singleton_L. eapply disjoint_singleton_r. by apply is_fresh.
-  - intros x. rewrite dom_singleton_L. intros ->%elem_of_singleton.
-    eapply lookup_insert.
-Qed.
-
-Lemma disjoint_strengthen T `{Countable T} (A1 A2 B1 B2 : gset T) : A1 ## B1 → A2 ⊆ A1 → B2 ⊆ B1 → A2 ## B2.
-Proof.
-  intros HD H1 H2.
-  apply elem_of_disjoint.
-  intros x HA HB.
-  edestruct (@elem_of_disjoint) as [HL _]; eapply HL.
-  - apply HD.
-  - eapply elem_of_weaken; first apply HA. done.
-  - eapply elem_of_weaken; first apply HB. done.
-Qed.
-
-Lemma extended_to_trans (χ1 χ2 χ3 : lloc_map) (ζ1 ζ2 : lstore) : 
-  extended_to χ1 ζ1 χ2 →
-  extended_to χ2 ζ2 χ3 →
-  extended_to χ1 (ζ1 ∪ ζ2) χ3 /\ ζ1 ##ₘ ζ2.
-Proof.
-  intros (HA1 & HA2 & HA3) (HB1 & HB2 & HB3). unfold extended_to; split_and!.
-  - split; last apply HB1. etransitivity; first apply HA1; apply HB1.
-  - erewrite dom_union_L. eapply disjoint_union_r. split; first done.
-    eapply disjoint_strengthen. 1: apply HB2. 2: done. apply subseteq_dom, HA1.
-  - intros γ. rewrite dom_union_L. intros [H|H]%elem_of_union; last by apply HB3.
-    eapply lookup_weaken; first by apply HA3.
-    apply HB1.
-  - eapply map_disjoint_dom. eapply disjoint_strengthen. 1: apply HB2. 2: done.
-    eapply extended_to_dom_subset; done.
-Qed.
-
-Lemma extended_to_trans_2 (χ1 χ2 χ3 : lloc_map) (ζ1 ζ2 : lstore) : 
-  extended_to χ1 ζ1 χ2 →
-  extended_to χ2 ζ2 χ3 →
-  extended_to χ1 (ζ2 ∪ ζ1) χ3 /\ ζ1 ##ₘ ζ2.
-Proof.
-  intros H1 H2.
-  destruct (extended_to_trans χ1 χ2 χ3 ζ1 ζ2) as (H3&H4). 1-2: done.
-  erewrite map_union_comm; done.
-Qed.
-
-Lemma extended_to_refl χ1 :
-  lloc_map_inj χ1 →
-  extended_to χ1 ∅ χ1.
-Proof.
-  by repeat split.
-Qed.
-
-Lemma extended_to_mono χ1 χ2 :
-  lloc_map_mono χ1 χ2 →
-  extended_to χ1 ∅ χ2.
-Proof.
-  intros (H1 & H2); by repeat split.
-Qed.
-
-Lemma is_val_extended_to_weaken χ1 χ2 ζ1 ζ2 v lv:
-  is_val χ1 ζ1 v lv →
-  extended_to χ1 ζ2 χ2 →
-  is_val χ2 (ζ1 ∪ ζ2) v lv.
-Proof.
-  intros H1 (H21&H22&H23).
-  eapply is_val_mono; last done.
-  1: apply H21.
-  apply map_union_subseteq_l.
-Qed.
-
-Lemma deserialize_ML_value χMLold v :  
-  lloc_map_inj χMLold
-→ ∃ χC ζimm lv,
-    extended_to χMLold ζimm χC
-  ∧ is_val χC ζimm v lv.
-Proof.
-  induction v as [[x|bo| |ℓ]| |v1 IHv1 v2 IHv2|v IHv|v IHv] in χMLold|-*; intros Hinj.
-  1-3,5: eexists χMLold, ∅, _; split_and!; [by eapply extended_to_refl | econstructor ].
-  Unshelve. 5: exact (Lloc 0). (* what happens for functions *)
-  - destruct (ensure_in_χ_pub χMLold ℓ) as (χ' & γ & Hχ' & Hγ & _); first done.
-    exists χ', ∅, (Lloc γ); (split_and!; last by econstructor).
-    by eapply extended_to_mono.
-  - destruct (IHv1 χMLold) as (χ1 & ζ1 & lv1 & Hext1 & Hlv1); first done.
-    destruct (IHv2 χ1) as (χ2 & ζ2 & lv2 & Hext2 & Hlv2); first by eapply extended_to_inj.
-    pose (Immut,(TagDefault,[lv1;lv2])) as blk.
-    edestruct (allocate_in_χ_priv χ2 blk) as (χ3 & γ & Hext3); first by eapply extended_to_inj.
-    eassert (extended_to χMLold _ χ3).
-    1: do 2 (eapply extended_to_trans; last done); done.
-    do 3 eexists; split; first done.
-    econstructor.
-    + rewrite lookup_union_r; first by erewrite lookup_singleton.
-      eapply map_disjoint_Some_r. 1: eapply extended_to_trans_2; first eapply extended_to_trans; done.
-      apply lookup_singleton.
-    + eapply is_val_extended_to_weaken; last done.
-      eapply is_val_extended_to_weaken; done.
-    + eapply is_val_extended_to_weaken; last done.
-      eapply is_val_mono; last done; try done.
-      eapply map_union_subseteq_r. eapply extended_to_trans; done.
-  - destruct (IHv χMLold) as (χ1 & ζ1 & lv1 & Hext1 & Hlv1); first done.
-    epose (Immut,(_,[lv1])) as blk.
-    edestruct (allocate_in_χ_priv χ1 blk) as (χ3 & γ & Hext3); first by eapply extended_to_inj.
-    eassert (extended_to χMLold _ χ3).
-    1: (eapply extended_to_trans; last done); done.
-    do 3 eexists; split; first done.
-    econstructor.
-    + rewrite lookup_union_r; first by erewrite lookup_singleton.
-      eapply map_disjoint_Some_r. 1: eapply extended_to_trans_2; done.
-      apply lookup_singleton.
-    + eapply is_val_extended_to_weaken; done.
-  - destruct (IHv χMLold) as (χ1 & ζ1 & lv1 & Hext1 & Hlv1); first done.
-    epose (Immut,(_,[lv1])) as blk.
-    edestruct (allocate_in_χ_priv χ1 blk) as (χ3 & γ & Hext3); first by eapply extended_to_inj.
-    eassert (extended_to χMLold _ χ3).
-    1: (eapply extended_to_trans; last done); done.
-    do 3 eexists; split; first done.
-    econstructor.
-    + rewrite lookup_union_r; first by erewrite lookup_singleton.
-      eapply map_disjoint_Some_r. 1: eapply extended_to_trans_2; done.
-      apply lookup_singleton.
-    + eapply is_val_extended_to_weaken; done.
-Qed.
-
-Lemma deserialize_ML_values χMLold vs :  
-  lloc_map_inj χMLold
-→ ∃ χC ζimm lvs,
-    extended_to χMLold ζimm χC
-  ∧ Forall2 (is_val χC ζimm) vs lvs.
-Proof.
-  induction vs as [|v vs IH] in χMLold|-*; intros Hinj.
-  - eexists χMLold, ∅, _; split_and!; [by eapply extended_to_refl | econstructor ].
-  - destruct (deserialize_ML_value χMLold v Hinj) as (χ1 & ζ1 & lv & Hext1 & Hlv1).
-    destruct (IH χ1) as (χ2 & ζ2 & lvs & Hext2 & Hlv2); first by eapply extended_to_inj.
-    eassert (extended_to χMLold _ χ2) by by eapply extended_to_trans.
-    eexists _, _, (lv::lvs). split_and!; first done.
-    econstructor.
-    + by eapply is_val_extended_to_weaken.
-    + eapply Forall2_impl; first done.
-      intros v' lv' H1. eapply is_val_mono; last done; try done.
-      eapply map_union_subseteq_r, extended_to_trans; done.
-Qed.
-
-Lemma deserialize_ML_block χMLold vs :  
-  lloc_map_inj χMLold
-→ ∃ χC ζimm blk,
-    extended_to χMLold ζimm χC
-  ∧ is_heap_elt χC ζimm vs blk.
-Proof.
-  intros H.
-  destruct (deserialize_ML_values χMLold vs H) as (χC & ζimm & lvs & H1 & H2).
-  by exists χC, ζimm, (Mut,(TagDefault,lvs)).
-Qed.
 
 
-Lemma is_store_blocks_mono_weaken χ1 χ2 ζ σ:
-  is_store_blocks χ1 ζ σ →
-  lloc_map_mono χ1 χ2 →
-  is_store_blocks χ2 ζ σ.
-Proof.
-  intros (H1&H2) [Hsub H3]. split.
-  - intros x Hx. destruct (H1 x Hx) as [y Hy]; exists y.
-    eapply lookup_weaken; done.
-  - intros γ; destruct (H2 γ) as [H2L H2R]; split.
-    + intros H; destruct (H2L H) as (ℓ&Vs&HH1&HH2). do 2 eexists; repeat split; try done.
-      eapply lookup_weaken; done.
-    + intros (ℓ&Vs&HH1&HH2).
-      apply H2R. do 2 eexists; repeat split; try done.
-      destruct (H1 ℓ) as (γ2&Hγ2); first by eapply elem_of_dom_2.
-      rewrite <- Hγ2.
-      eapply lookup_weaken in Hγ2; last done.
-      f_equiv. eapply H3; done.
-Qed.
-
-Lemma is_heap_elt_weaken χ ζ vs blk ζ' χ' :
-  is_heap_elt χ ζ vs blk
-→ χ ⊆ χ'
-→ ζ ⊆ ζ'
-→ is_heap_elt χ' ζ' vs blk.
-Proof.
-  intros H1 H2 H3.
-  inversion H1; subst.
-  econstructor. eapply Forall2_impl; first done.
-  intros x y H4; eapply is_val_mono; last done. all:done.
-Qed.
-
-Lemma is_heap_elt_weaken_2 χ ζ vs blk ζ' χ' :
-  is_heap_elt χ ζ vs blk
-→ extended_to χ' ζ χ
-→ dom ζ' ⊆ dom χ'
-→ is_heap_elt χ (ζ' ∪ ζ) vs blk.
-Proof.
-  intros H1 H2 H3.
-  eapply is_heap_elt_weaken. 1: done.
-  1: done. eapply map_union_subseteq_r.
-  eapply map_disjoint_dom. eapply disjoint_strengthen.
-  1: apply H2. 1-2:done.
-Qed.
-
-Lemma deserialize_ML_heap χMLold σ : 
-  lloc_map_inj χMLold
-→ ∃ χC ζσ ζnewimm,
-    extended_to χMLold ζnewimm χC
-  ∧ is_store_blocks χC σ ζσ
-  ∧ is_store χC (ζσ ∪ ζnewimm) σ.
-Proof.
-  revert χMLold.
-  induction σ as [|ℓ [vv|] σ Hin IH] using map_ind; intros χMLold HχMLold .
-  - exists χMLold, ∅, ∅; split_and!. 2: econstructor.
-    + by eapply extended_to_refl.
-    + intros γ; rewrite dom_empty_L; done.
-    + split; rewrite dom_empty_L. 1: done.
-      intros (ℓ & Vs & H1 & H2). exfalso. rewrite lookup_empty in H2. done.
-    + intros ℓ Vs γ blk Hc. exfalso. rewrite lookup_empty in Hc. done.
-  - destruct (IH χMLold) as (χ0 & ζσ & ζi0 & Hext & Hstbl & Hstore). 1: done.
-    destruct (ensure_in_χ_pub χ0 ℓ) as (χ1 & γ & Hχ1 & Hγ & Hold); first by eapply extended_to_inj.
-    apply extended_to_mono in Hχ1.
-    destruct (deserialize_ML_block χ1 vv) as (χ2 & ζi2 & lvs & Hext2 & Helt); first by eapply extended_to_inj.
-    edestruct (extended_to_trans) as (HextA&Hdisj1). 1: exact Hext. 1: eapply extended_to_trans; done.
-    rewrite map_empty_union in Hdisj1.
-    rewrite map_empty_union in HextA.
-    assert (is_store_blocks χ2 (<[ℓ:=Some vv]> σ) (<[γ:=lvs]> ζσ)) as Hstore2.
-    1: {eapply is_store_blocks_restore_loc.
-        * eapply is_store_blocks_mono_weaken; first done. eapply extended_to_trans; done.
-        * apply Hext2.
-        * eapply lookup_weaken. 1: done. apply Hext2.
-        * by right. }
-    assert (dom (<[γ:=lvs]> ζσ ∪ ζi0) ⊆ dom χ1) as Hsub3.
-    { rewrite dom_union_L. eapply union_subseteq. split.
-      * rewrite dom_insert_L. apply union_subseteq. split.
-        eapply singleton_subseteq_l; first by eapply elem_of_dom_2.
-        eapply elem_of_subseteq; intros k Hk.
-        destruct Hstbl as (HH1&HH2). apply HH2 in Hk. destruct Hk as (?&?&H1&H2).
-        eapply elem_of_dom_2. eapply lookup_weaken; first apply H1.
-        eapply Hχ1.
-      * etransitivity; last eapply subseteq_dom, Hχ1.
-        eapply extended_to_dom_subset; done. }
-    eexists χ2, (<[γ := lvs]> ζσ), (ζi0 ∪ ζi2). split_and!. 1-2:done.
-    + intros ℓ' vs γ' blk H1 H2 H3.  destruct HextA as (HH1&HH2&HH3).
-      apply lookup_union_Some in H3. 1: destruct H3 as [H3|H3].
-      3: { eapply map_disjoint_dom; eapply elem_of_disjoint.
-           intros x Hx1 Hx2; specialize (HH3 x Hx2). destruct Hstore2 as [HHL HHR].
-           apply HHR in Hx1. destruct Hx1 as (l1 & Vs1 & ? & ?); congruence. }
-      2: { rewrite HH3 in H2; last by eapply elem_of_dom_2. congruence. }
-      apply lookup_insert_Some in H3. destruct H3 as [[? ?]|[Hne H3]].
-      * subst. rewrite map_union_assoc.
-        eapply lookup_weaken in Hγ. 2: eapply Hext2. rewrite Hγ in H2. injection H2; intros ->.
-        rewrite lookup_insert in H1. injection H1; intros ->.
-        by eapply is_heap_elt_weaken_2.
-      * eapply lookup_insert_Some in H1. destruct H1 as [[-> H]|[Hne1 H1]].
-        1: {exfalso. apply Hne. eapply HH1. 2: done. eapply lookup_weaken; first done. apply Hext2. }
-        assert (χ0 !! γ' = Some (LlocPublic ℓ')) as H2'.
-        1: {destruct Hstbl as [HHL HHR]. destruct (HHL ℓ') as (gg&Hgg); first by eapply elem_of_dom_2.
-            rewrite <- Hgg; f_equal. eapply HH1. 1: done. eapply lookup_weaken; first done. etransitivity; last eapply Hext2; eapply Hχ1. }
-        eapply is_heap_elt_weaken.
-        1: eapply Hstore. 1: done. 3: etransitivity; first eapply Hχ1; last apply Hext2.
-        2: erewrite lookup_union_l; first done. 1: done.
-        1: eapply not_elem_of_dom; intros H; eapply Hext in H; congruence.
-        etransitivity; first eapply map_union_mono_l.
-        2: etransitivity; first eapply map_union_mono_r. 4: done.
-        1: eapply map_union_subseteq_l.
-        1: eapply is_store_blocks_is_private_blocks_disjoint; done.
-        eapply insert_subseteq, not_elem_of_dom.
-        intros H. destruct Hstbl as [HHL HHR]. eapply HHR in H.
-        destruct H as (?&?&Heq1&HeqF). eapply lookup_weaken in Heq1; first erewrite Hγ in Heq1. 2: apply Hχ1.
-        injection Heq1; intros ->; rewrite HeqF in Hin; congruence.
-  - destruct (IH χMLold) as (χ0 & ζσ & ζi0 & Hext & Hstbl & Hstore). 1: done.
-    destruct (ensure_in_χ_pub χ0 ℓ) as (χ1 & γ & Hχ1 & Hγ & Hold); first by eapply extended_to_inj.
-    edestruct (extended_to_trans) as (HextA&Hdisj1); first exact Hext. 1: eapply extended_to_mono, Hχ1.
-    exists χ1, ζσ, ζi0. split_and!. 2: destruct Hstbl as [HL HR]; split.
-    + rewrite map_union_empty in HextA. done.
-    + rewrite dom_insert_L. intros ℓ0 [->%elem_of_singleton|H]%elem_of_union.
-      1: eexists; done.
-      destruct (HL ℓ0 H) as (γ1&Hγ1). exists γ1; eapply lookup_weaken; first done.
-      eapply Hχ1.
-    + intros γ0; specialize (HR γ0) as (HRL&HRR). split.
-      1: intros H; destruct (HRL H) as (ℓ0 & Vs & H3 & H5); do 2 eexists;
-        split; first (eapply lookup_weaken; first done; eapply Hχ1);
-        rewrite lookup_insert_ne; first done;
-        intros ->; rewrite Hin in H5; congruence.
-      intros (ℓ0&Vs&HH1&HH2).
-      rewrite lookup_insert_Some in HH2; destruct HH2 as [[? ?]|[Hne HH2]].
-      1: congruence.
-      eapply HRR. eexists ℓ0, Vs. split; last done.
-      eapply elem_of_dom_2 in HH2.
-      destruct (HL ℓ0 HH2) as (γ1&Hγ1). rewrite <- Hγ1. f_equal.
-      eapply Hχ1; try done. eapply lookup_weaken, Hχ1; done.
-    + intros ℓ1 vs γ1 blk [[? ?]|[? H1]]%lookup_insert_Some H2 H3; try congruence.
-      eapply is_heap_elt_weaken. 1: eapply Hstore; try done.
-      3: done. 2: eapply Hχ1.
-      destruct Hstbl as [HHL HHR].
-      destruct (HHL ℓ1) as (k1&Hk1); first by eapply elem_of_dom_2.
-      rewrite <- Hk1. f_equal. eapply Hχ1; try done. eapply lookup_weaken, Hχ1; done.
-Qed.
-
-Lemma deserialize_ML_heap_extra ζMLold χMLold σ : 
-  lloc_map_inj χMLold
-→ dom ζMLold ⊆ dom χMLold
-→ (map_Forall (fun _ ℓ => σ !! ℓ = Some None) (pub_locs_in_lstore χMLold ζMLold))
-→ ∃ χC ζσ ζnewimm,
-    extended_to χMLold ζnewimm χC
-  ∧ is_store_blocks χC σ ζσ
-  ∧ ζMLold ##ₘ (ζσ ∪ ζnewimm)
-  ∧ is_store χC (ζMLold ∪ ζσ ∪ ζnewimm) σ.
-Proof.
-  intros H1 H2 H3.
-  destruct (deserialize_ML_heap χMLold σ) as (χC&ζσ&ζi&HA1&HA2&HA3). 1: apply H1.
-  assert (ζMLold ##ₘ ζσ ∪ ζi) as Hdisj.
-  1: eapply map_disjoint_union_r; split; last (eapply map_disjoint_dom, disjoint_strengthen; first apply HA1; done).
-  1: { eapply map_disjoint_spec. intros γ b1 b2 HH1 HH2.
-       destruct HA2 as [_ HA2R]. eapply elem_of_dom_2 in HH2. apply HA2R in HH2.
-       destruct HH2 as (ℓ & Vs & HH7 & HH8).
-       erewrite (map_Forall_lookup_1 _ _ _ _ H3) in HH8.
-       2: { eapply elem_of_dom_2 in HH1. erewrite pub_locs_in_lstore_lookup; first done; first done.
-            eapply elem_of_weaken in H2; last done.
-            eapply elem_of_dom in H2; destruct H2 as [k Hk]. rewrite Hk. 
-            eapply lookup_weaken in Hk; first erewrite HH7 in Hk. 2: eapply HA1. done. }
-       congruence. }
-  do 3 eexists; split_and!; try done.
-  - intros ℓ vs γ b He1 He2 He3.
-    eapply is_heap_elt_weaken. 1: eapply HA3; try done. 2: done.
-    + rewrite <- map_union_assoc in He3. eapply lookup_union_Some in He3; destruct He3; try done.
-      destruct (HA2) as [HL HR]. destruct (HR γ) as [HRL HRR]. eapply elem_of_dom in HRR. destruct HRR as [vv Hvv].
-      2: do 2 eexists; done.
-      exfalso. erewrite map_disjoint_Some_r in H; try congruence. 1: done.
-      erewrite lookup_union_Some_l; last done; first done.
-    + erewrite <- map_union_assoc. eapply map_union_subseteq_r. done.
-Qed.
-
-Lemma collect_dom_θ_vs (θdom : gset lloc) (vs : list lval) : exists θdom' : gset lloc, forall γ, (Lloc γ ∈ vs ∨ γ ∈ θdom) ↔ γ ∈ θdom'.
-Proof.
-  induction vs as [|[|ℓ] vs (θdom1 & IH)].
-  - exists θdom. intros γ. split; last eauto. intros [[]%not_elem_of_nil|?]; done.
-  - exists θdom1. intros γ. split.
-    + intros [[Hc|H]%elem_of_cons|?]; try congruence; apply IH. 1: by left. by right.
-    + intros [H|H]%IH; last by right. left. right. done.
-  - exists (θdom1 ∪ {[ ℓ ]}). intros γ. split.
-    + intros [[Hc|H]%elem_of_cons|?]; eapply elem_of_union. 1: right; eapply elem_of_singleton; congruence.
-      all: left; apply IH. 1: by left. by right.
-    + intros [[H|H]%IH| ->%elem_of_singleton]%elem_of_union. 1: left; right; done. 1: right; done.    
-      left; left; done.
-Qed.
-
-Lemma collect_dom_θ_ζ_blocks (θdom : gset lloc) (ζ : lstore) : exists θdom' : gset lloc,
-    forall γ, ((exists γ1 m t vs, ζ !! γ1 = Some (m, (t, vs)) ∧ Lloc γ ∈ vs) ∨ γ ∈ θdom) ↔ γ ∈ θdom'.
-Proof.
-  induction ζ as [|k [m [t vs]] ζ Hne (θdom1 & Hdom1)] using map_ind.
-  - exists θdom; split.
-    + intros [(γ1&m&t&vs&H1&H2)|Hold]; last done.
-      rewrite lookup_empty in H1; done.
-    + intros H; by right.
-  - destruct (collect_dom_θ_vs θdom1 vs) as (θdom2 & Hdom2).
-    exists θdom2. intros γ; split.
-    + intros [(γ1&m'&t'&vs'&[[-> Hinj]|[Hne2 Hin]]%lookup_insert_Some&H2)|Hold].
-      1: apply Hdom2; left; congruence.
-      1: apply Hdom2; right; apply Hdom1; left; by repeat eexists.
-      1: apply Hdom2; right; apply Hdom1; right; done.
-    + intros [H|[(γ1&m'&t'&vs'&H1&H2)|H]%Hdom1]%Hdom2.
-      1: left; do 4 eexists; split; first eapply lookup_insert; done.
-      2: by right.
-      left; do 4 eexists; split; last done; first rewrite lookup_insert_ne; first done.
-      intros ->; rewrite Hne in H1; congruence.
-Qed.
-
-Lemma collect_dom_θ_ζ (θdom : gset lloc) (ζ : lstore) : exists θdom' : gset lloc,
-    forall γ, (γ ∈ dom ζ ∨ (exists γ1 m t vs, ζ !! γ1 = Some (m, (t, vs)) ∧ Lloc γ ∈ vs) ∨ γ ∈ θdom) ↔ γ ∈ θdom'.
-Proof.
-  destruct (collect_dom_θ_ζ_blocks θdom ζ) as (θdom1 & Hdom1).
-  exists (dom ζ ∪ θdom1). intros γ; split.
-  - (intros [H|H]; apply elem_of_union); first by left.
-    right; apply Hdom1; done.
-  - intros [H|H]%elem_of_union; first by left. right; by apply Hdom1.
-Qed.
-
-Lemma collect_dom_θ_roots (θdom : gset lloc) (roots : roots_map) : exists θdom' : gset lloc,
-    forall γ, ((exists k, roots !! k = Some (Lloc γ)) ∨ γ ∈ θdom) ↔ γ ∈ θdom'.
-Proof.
-  induction roots as [|k [z|l] roots Hne (θdom1 & IH)] using map_ind.
-  - exists θdom. intros γ. split; last eauto. intros [[? H%lookup_empty_Some]|?]; done.
-  - exists θdom1. intros γ. split.
-    + intros [[k1 [[-> ?]|[H1 H2]]%lookup_insert_Some]|?]; try congruence; apply IH. 2: by right. left. by eexists.
-    + intros [[k' Hk]|H]%IH; last by right. left. exists k'. rewrite lookup_insert_ne; first done. intros ->; rewrite Hne in Hk; done.
-  - exists (θdom1 ∪ {[ l ]}). intros γ. split.
-    + intros [[k1 [[-> ?]|[H1 H2]]%lookup_insert_Some]|?]; try congruence; eapply elem_of_union. 1: right; eapply elem_of_singleton; congruence.
-      all: left; apply IH. 2: by right. left; by eexists.
-    + intros [[[k' Hk]|H]%IH| ->%elem_of_singleton]%elem_of_union. 2: by right. 2: left; exists k; by rewrite lookup_insert.
-      left; exists k'; rewrite lookup_insert_ne; first done. intros ->; rewrite Hne in Hk; congruence.
-Qed.
-
-Lemma injectivify_map (S : gset lloc) : exists M : addr_map, dom M = S ∧ gmap_inj M.
-Proof.
-  induction S as [|s S Hne (M & <- & Hinj)] using set_ind_L.
-  - exists ∅; split; first by rewrite dom_empty_L. intros ??? H1; exfalso. rewrite lookup_empty in H1; done.
-  - exists (<[s := fresh (codom M)]> M). split.
-    1: by rewrite dom_insert_L.
-    apply gmap_inj_extend; try done.
-    intros k' v' H%codom_spec_2 <-. unshelve eapply is_fresh; last exact H. all: apply _.
-Qed.
-
-Lemma find_repr_lval_vv θ v : 
-   (forall γ, Lloc γ = v → γ ∈ dom θ)
- → exists l, repr_lval θ v l.
-Proof.
-  intros H. destruct v as [z|a].
-  - eexists; by econstructor.
-  - destruct (θ !! a) as [va|] eqn:Heq.
-    2: eapply not_elem_of_dom in Heq; exfalso; apply Heq; apply H; done.
-    eexists; econstructor; apply Heq.
-Qed.
-
-Lemma find_repr_lval_vs θ vs : 
-   (forall γ, Lloc γ ∈ vs → γ ∈ dom θ)
- → exists ls, Forall2 (repr_lval θ) vs ls.
-Proof.
-  intros H; induction vs as [|v vs IH] in H|-*.
-  - exists nil. econstructor.
-  - destruct IH as [ls IH]; first (intros γ Hγ; eapply H; right; done).
-    destruct (find_repr_lval_vv θ v) as [l Hl].
-    1: intros γ <-; apply H; by left.
-    eexists. econstructor; done.
-Qed.
-
-Lemma find_repr_roots θ roots privmem : 
-   roots_are_live θ roots
- → dom privmem ## dom roots
- → exists mem, repr θ roots privmem mem.
-Proof.
-  revert privmem. unfold repr.
-  induction roots as [|l a roots_m Hin IH] using map_ind; intros privmem Hlive Hdisj.
-  - exists privmem, ∅. split_and!.
-    + econstructor.
-    + eapply map_disjoint_empty_r.
-    + by rewrite map_empty_union.
-  - destruct (IH privmem) as (mem1 & memr1 & Hrepr1 & Hdisj1 & Heq1).
-    1: { intros a1 w1 H1; eapply Hlive; rewrite lookup_insert_ne; first done.
-         intros ->; rewrite Hin in H1; congruence. }
-    1: rewrite dom_insert_L in Hdisj; set_solver.
-    destruct (find_repr_lval_vv θ a) as (w & Hw).
-    1: intros γ <-; eapply Hlive; apply lookup_insert.
-    exists (<[l:=Storing w]> mem1), (<[l:=Storing w]> memr1). split_and!.
-    + econstructor. 1: done. 1:done. 2: erewrite <- repr_roots_dom; last apply Hrepr1. all: by eapply not_elem_of_dom.
-    + apply map_disjoint_dom in Hdisj1. apply map_disjoint_dom.
-      rewrite dom_insert_L. rewrite dom_insert_L in Hdisj. set_solver.
-    + erewrite Heq1. now rewrite insert_union_l.
-Qed.
-
-
-Lemma set_to_some θ mem roots_m privmem :
-    repr θ roots_m privmem mem
- -> gen_heap_interp (privmem ∪ ((λ _ : lval, None) <$> roots_m))
- -∗ ([∗ set] a0 ∈ dom roots_m, a0 O↦ None)
- ==∗ gen_heap_interp mem
-     ∗ ([∗ map] a0↦v0 ∈ roots_m, ∃ w, a0 ↦C{DfracOwn 1} w ∗ ⌜repr_lval θ v0 w⌝).
-Proof.
-  intros (mm & Hrepr1 & Hrepr2 & Hrepr3).
-  induction Hrepr1 in Hrepr2,Hrepr3,mem,privmem|-*.
-  + iIntros "Hheap Hset !>".
-    rewrite fmap_empty. rewrite dom_empty_L. rewrite map_union_empty.
-    rewrite map_empty_union in Hrepr3. subst mem. iFrame.
-    iApply big_sepM_empty. done.
-  + eapply not_elem_of_dom in H0,H1. iIntros "Hheap Hset".
-    rewrite dom_insert_L.
-    iPoseProof (big_sepS_insert) as "(Hb1 & _)"; first eapply not_elem_of_dom_2, H0.
-    iPoseProof ("Hb1" with "Hset") as "(Hw & Hset)".
-    rewrite fmap_insert. rewrite <- insert_union_r.
-    2: eapply map_disjoint_Some_r; first done; by rewrite lookup_insert.
-    iMod (gen_heap_update _ _ _ (Storing w) with "Hheap Hw") as "(Hheap & Hw)".
-    rewrite insert_insert.
-    rewrite insert_union_l.
-    iMod (IHHrepr1 with "Hheap Hset") as "(Hheap & Hset)".
-    * eapply map_disjoint_insert_l_2; first done.
-      erewrite <- (delete_insert mem0); last done.
-      by eapply map_disjoint_delete_r.
-    * done.
-    * rewrite <- insert_union_r; last done.
-      subst mem. rewrite insert_union_l. iModIntro.
-      iFrame.
-      iApply (big_sepM_insert_2 with "[Hw] Hset").
-      iExists w. iFrame. done.
-Qed.
-
-Lemma zip_args_length a b : length a = length b → exists v, C_lang.zip_args a b = Some v.
-Proof.
-  intros Hlen.
-  assert (Forall2 (fun _ _ => True) a b) as Hforall by by apply Forall2_true.
-  clear Hlen. induction Hforall as [|[|s] ar bx br _ Hforall [v IH]].
-  - cbn. eexists _; done.
-  - cbn. eexists; apply IH.
-  - eexists. cbn. rewrite IH. cbn. done.
-Qed.
-
-Lemma apply_function_arity F ws : arity F = length ws → ∃ k, C_lang.apply_function F ws = Some k.
-Proof.
-  intros H. destruct F as [c args]. cbn in H|-*.
-  destruct (zip_args_length c ws) as [σ Hσ]; first done.
-  eexists; rewrite Hσ. done.
-Qed.
 
 Lemma run_function_correct F (vv : list ML_lang.val) T E Φ: 
     ⌜arity F = length vv⌝
@@ -848,13 +199,13 @@ Proof.
 
     destruct (deserialize_ML_heap_extra (ζML ρml) (χML ρml) σ) as (χ1 & ζσ & ζσimm & Hext & Hstorebl & Hdisj & Hstore).
     1: done.
-    1: eapply elem_of_subseteq; done.
+    1: done.
     1: done.
     destruct (deserialize_ML_values χ1 vv) as (χ2 & ζimm & lvs & Hext2 & Hvs).
     1: apply Hext.
 
     assert (ζML ρml ∪ ζσ ∪ ζσimm ##ₘ ζimm) as Hdis1.
-    1: { eapply map_disjoint_dom. eapply disjoint_strengthen. 1: eapply Hext2. 2: done.
+    1: { eapply map_disjoint_dom. eapply disjoint_weaken. 1: eapply Hext2. 2: done.
          rewrite dom_union_L. eapply union_subseteq. split. 2: by eapply extended_to_dom_subset.
          rewrite dom_union_L. eapply union_subseteq; split.
          1: etransitivity; first by eapply elem_of_subseteq. 1: eapply subseteq_dom, Hext.
@@ -868,7 +219,7 @@ Proof.
     destruct (injectivify_map θdom3) as (θC & Hdom & Hinj).
     destruct (find_repr_lval_vs θC lvs) as (ws & Hws).
     1: intros γ Hγ; subst θdom3; apply Hθdom3; right; apply Hθdom2; left; done.
-    destruct (apply_function_arity F ws) as (ec & Hec).
+    destruct (apply_function_arity F ws) as (HL&_); destruct HL as (ec&Hec).
     1: rewrite Harity; etransitivity; eapply Forall2_length; done.
     assert (roots_are_live θC (rootsML ρml)) as Hrootslive.
     1: { intros a γ H1. subst θdom3. apply Hθdom3. left. by eexists. }
@@ -886,7 +237,7 @@ Proof.
          1: by eapply Hext. 2: by eapply Hext2. 2: done. 1: apply Hext2. }
     1: { reflexivity. }
     1: { rewrite map_union_assoc. apply map_disjoint_union_r_2. 1: done.
-         eapply map_disjoint_dom, disjoint_strengthen; first eapply map_disjoint_dom, Hdis1; try done.
+         eapply map_disjoint_dom, disjoint_weaken; first eapply map_disjoint_dom, Hdis1; try done.
          erewrite ! dom_union_L; set_solver. }
     1: { intros ℓ vs γ b H1 H2 H3. unfold ζC in *. rewrite ! map_union_assoc. rewrite ! map_union_assoc in H3.
          apply lookup_union_Some_inv_l in H3.
@@ -957,10 +308,14 @@ Proof.
            intros γ v1 v2 H1 H2. rewrite H1 in H2. injection H2; intros ->. econstructor. }
       1: apply H3.
       1: done.
-    * iApply (wp_simulates with "Hnb"); iApply ("Hwp" with "[- ] [] [] Hsim"); try done.
+    * iApply (wp_simulates with "Hnb").
+      iApply ("Hwp" with "[-] [] [] Hsim"); try done.
       unfold GC; cbn.
       iExists (dom (rootsML ρml)), (rootsML ρml).
-      iFrame "HAGCθ HAGCbound HArootss HArootsm Hrootspto". done.
+      iFrame. done.
 Qed.
 
 End Simulation.
+
+
+
