theories/interop/wrapper_wp_ext_call_laws.v
@@ -1,0 +1,181 @@
+From Coq Require Import ssreflect.
+From stdpp Require Import strings gmap.
+From melocoton Require Import named_props.
+From melocoton.mlanguage Require Import mlanguage.
+From melocoton.language Require Import language weakestpre.
+From melocoton.mlanguage Require Import weakestpre.
+From melocoton.interop Require Import wrappersem basics_resources wrapperstate.
+From iris.base_logic.lib Require Import ghost_map ghost_var gset_bij.
+From iris.algebra Require Import gset gset_bij.
+From melocoton Require Import big_sepM_limited.
+From iris.proofmode Require Import proofmode.
+From melocoton.ml_toy_lang Require Import lang melocoton.lang_instantiation melocoton.primitive_laws.
+From melocoton.c_toy_lang Require Import lang melocoton.lang_instantiation melocoton.primitive_laws notation.
+From melocoton.interop Require Import linking_wp basics wrapper_wp wrapper_wp_block_sim wrapper_wp_utils.
+Import Wrap.
+
+Section Laws.
+
+Context {hlc : has_lc}.
+Context {Σ : gFunctors}.
+Context `{!heapGS_ML Σ, !heapGS_C Σ}.
+Context `{!invGS_gen hlc Σ}.
+Context `{!wrapperGS Σ}.
+
+Context (p : language.prog C_lang).
+Context (Hforbid : Forall (fun k => p !! k = None) forbidden_function_names).
+
+Notation MLval := ML_lang.val.
+Notation Cval := C_lang.val.
+
+Implicit Types P : iProp Σ.
+Import mlanguage.
+
+
+Notation mkPeC p T := ({| penv_prog := p; penv_proto := T |} : prog_environ _ Σ).
+Notation mkPeW p T := ({| weakestpre.penv_prog := p; weakestpre.penv_proto := T |} : weakestpre.prog_environ wrap_lang Σ).
+
+Notation wrap_return := (fun Φ (a:Cval) => (∃ θ' l v, GC θ' ∗ Φ v ∗ ⌜repr_lval θ' l a⌝ ∗ block_sim v l)%I).
+(* TODO move store / load somewhere else *)
+Lemma store_to_root E (l:loc) (v v' : lval) w θ :
+  {{{GC θ ∗ l ↦roots v' ∗ ⌜repr_lval θ v w⌝}}}
+     (#l <- w)%E @ (mkPeC p WP_ext_call_spec); E
+  {{{ RET LitV LitUnit; l ↦roots v ∗ GC θ }}}.
+Proof.
+  iIntros (Φ) "(HGC&Hroots&%Hrepr) HΦ".
+  iNamed "HGC".
+  iPoseProof (ghost_map_lookup with "HArootsm Hroots") as "%H".
+  iPoseProof (big_sepM_delete) as "(HL&_)"; first apply H.
+  iPoseProof ("HL" with "Hrootspto") as "((%w'&Hown&%Hrepr2) & Hrp)"; iClear "HL".
+  iMod (ghost_map_update with "HArootsm Hroots") as "(HArootsm&Hroots)".
+  iApply (wp_store with "Hown").
+  iIntros "!> Hown". iApply "HΦ".
+  iFrame "Hroots".
+  do 2 iExists _.
+  iFrame.
+  rewrite dom_insert_lookup_L; last done. iSplitR; first done.
+  iSplitR.
+  - iPureIntro. intros l' γ [[-> ->]|[Hne HH]]%lookup_insert_Some.
+    2: by eapply Hrootslive.
+    inversion Hrepr; subst. by eapply elem_of_dom_2.
+  - iPoseProof (big_sepM_insert_delete) as "(_&HR)"; iApply "HR"; iClear "HR".
+    iSplitL "Hown"; last done.
+    iExists w. iFrame. done.
+Qed.
+
+Lemma load_from_root E (l:loc) (v : lval) dq θ :
+  {{{GC θ ∗ l ↦roots{dq} v}}}
+     ( * #l)%E @ (mkPeC p WP_ext_call_spec); E
+  {{{ w, RET w; l ↦roots{dq} v ∗ GC θ ∗ ⌜repr_lval θ v w⌝ }}}.
+Proof.
+  iIntros (Φ) "(HGC&Hroot) HΦ".
+  iNamed "HGC".
+  iPoseProof (ghost_map_lookup with "HArootsm Hroot") as "%H".
+  iPoseProof (big_sepM_delete) as "(HL&HR)"; first apply H.
+  iPoseProof ("HL" with "Hrootspto") as "((%w&Hown&%Hrepr2) & Hrp)"; iClear "HL".
+  iApply (wp_load with "Hown").
+  iIntros "!> Hown". iApply "HΦ".
+  iFrame "Hroot". iSplitL; last done.
+  iPoseProof ("HR" with "[Hown Hrp]") as "Hrootsm"; iClear "HR".
+  - iFrame. iExists w; by iFrame.
+  - do 2 iExists _. iFrame. done.
+Qed.
+
+
+Notation fillCCall K s vv := (language.fill K (language.of_class C_lang (ExprCall s (vv:list Cval)))).
+
+Definition ext_call_is_sound (Hspec : string -d> list Cval -d> (Cval -d> iPropO Σ) -d> iPropO Σ) :=
+  forall E T s (vv:list Cval) K Ξ Φ,
+    ⌜p !! s = None⌝
+ -∗ not_at_boundary
+ -∗ Hspec s vv Ξ
+ -∗ ▷ (∀ r, Ξ r -∗ not_at_boundary -∗ WP (ExprC (language.fill K (language.of_class C_lang (ExprVal r)))) @ (mkPeW (p : prog wrap_lang) T); E {{v, Φ v }})
+ -∗ WP (ExprC (fillCCall K s vv)) @ (mkPeW (p : prog wrap_lang) T); E {{ v, Φ v}}.
+
+
+Lemma wp_ext_call_int2val : ext_call_is_sound WP_int2val_spec.
+Proof.
+  intros E T s vv K Ξ Φ.
+  rewrite weakestpre.wp_unfold. rewrite /weakestpre.wp_pre.
+  iIntros "%Hnone Hnb HT IH %σ Hσ".
+  destruct σ as [ρml σ | ρc mem].
+  1: iExFalso; iNamed "Hσ"; iNamed "SIML"; iPoseProof (ghost_var_agree with "Hnb HAbound") as "%HH"; congruence.
+  iNamed "Hσ"; iNamed "SIC".
+  cbn. unfold WP_int2val_spec. iNamed "HT". iNamed "HGC".
+    iPoseProof (ghost_var_agree with "HAGCθ HAθ") as "%H"; subst θ.
+    iModIntro. iRight. iRight. iSplitR.
+    + iPureIntro. econstructor. eapply head_prim_step.
+      eapply (PrimInt2valS _ _ _ _ _ _ _ (fun k => True)).
+      2: econstructor. 2: done.
+      cbn. done.
+    + iIntros (X Hstep).
+      destruct Hstep as ([] & x & Hre & Hstep). change (fill () x) with x in Hre. subst x.
+      cbn in Hstep; unfold step,mrel in Hstep; cbn in Hstep.
+      inversion_call_step Hstep ([ #z]).
+      do 3 iModIntro.
+      do 2 iExists _. change (Wrap.fill () ?x) with (x) in H5.
+      iSplitR; first (iPureIntro; eapply H5).
+      iSplitR "Hnb IH HWP HAGCθ HAGCbound HArootss HArootsm Hrootspto".
+      * cbn. unfold C_state_interp. iSplitL "HσC HnC"; first (iExists nCv; iFrame).
+        repeat iExists _. iFrame. iSplitL; first by iExists _. iPureIntro; done.
+      * iApply ("IH" with "[-Hnb] Hnb").
+        iApply ("HWP" with "[-]"); last done.
+        do 2 iExists _; iFrame. done.
+Qed.
+
+Lemma wp_ext_call_val2int : ext_call_is_sound WP_val2int_spec.
+Proof.
+  intros E T s vv K Ξ Φ.
+  rewrite weakestpre.wp_unfold. rewrite /weakestpre.wp_pre.
+  iIntros "%Hnone Hnb HT IH %σ Hσ".
+  destruct σ as [ρml σ | ρc mem].
+  1: iExFalso; iNamed "Hσ"; iNamed "SIML"; iPoseProof (ghost_var_agree with "Hnb HAbound") as "%HH"; congruence.
+  iNamed "Hσ"; iNamed "SIC".
+  cbn. unfold WP_val2int_spec. iNamed "HT". iNamed "HGC".
+    iPoseProof (ghost_var_agree with "HAGCθ HAθ") as "%H"; subst θ.
+    iModIntro. iRight. iRight. iSplitR.
+    + iPureIntro. econstructor. eapply head_prim_step.
+      eapply (PrimVal2intS _ _ _ _ _ _ _ (fun k => True)). 2: apply Hrepr. all:done.
+    + iIntros (X Hstep).
+      destruct Hstep as ([] & x & Hre & Hstep). change (fill () x) with x in Hre. subst x.
+      cbn in Hstep; unfold step,mrel in Hstep; cbn in Hstep.
+      inversion_call_step Hstep ([w]).
+      do 3 iModIntro.
+      do 2 iExists _. change (Wrap.fill () ?x) with (x) in H5.
+      iSplitR; first (iPureIntro; eapply H5).
+      iSplitR "Hnb IH HWP HAGCθ HAGCbound HArootss HArootsm Hrootspto".
+      * cbn. unfold C_state_interp. iSplitL "HσC HnC"; first (iExists nCv; iFrame).
+        repeat iExists _. iFrame. iSplitL; first by iExists _. iPureIntro; done.
+      * iApply ("IH" with "[-Hnb] Hnb"). inversion Hrepr; inversion H4; subst; rewrite ! H10.
+        iApply ("HWP").
+        do 2 iExists _; iFrame. done.
+Qed.
+
+Ltac solve_ext_call H := 
+    iPoseProof (H with "[] Hnb H [IH]") as "Hwp"; [done
+    | iIntros "!> %r HΞ Hnb"; iApply ("IH" with "HΞ Hnb"); by iApply "Hr"
+    | rewrite weakestpre.wp_unfold; rewrite /weakestpre.wp_pre;
+      iApply ("Hwp" $! (CState _ _));
+      iSplitL "HσC HnC"; first (iExists _; iFrame);
+      unfold C_state_interp, named; do 5 iExists _ ;
+      iFrame;
+      (iSplitL "HAnMLv"; first by iExists _); done ].
+
+Lemma wp_ext_call_collect_all : ext_call_is_sound WP_ext_call_spec.
+Proof.
+  intros E T s vv K Ξ Φ.
+  rewrite weakestpre.wp_unfold. rewrite /weakestpre.wp_pre.
+  iIntros "%Hnone Hnb HT IH %σ Hσ".
+  destruct σ as [ρml σ | ρc mem].
+  1: iExFalso; iNamed "Hσ"; iNamed "SIML"; iPoseProof (ghost_var_agree with "Hnb HAbound") as "%HH"; congruence.
+  iNamed "Hσ"; iNamed "SIC".
+  cbn. iDestruct "HT" as "[H|H]".
+  - solve_ext_call wp_ext_call_int2val.
+  - solve_ext_call wp_ext_call_val2int.
+Qed.
+
+
+End Laws.
+
+
+
