theories/interop/wrapper_wp_utils.v
@@ -1,0 +1,745 @@
+From Coq Require Import ssreflect.
+From stdpp Require Import strings gmap.
+From melocoton Require Import named_props.
+From melocoton.mlanguage Require Import mlanguage.
+From melocoton.language Require Import language weakestpre.
+From melocoton.mlanguage Require Import weakestpre.
+From melocoton.interop Require Import wrappersem basics_resources wrapperstate.
+From iris.base_logic.lib Require Import ghost_map ghost_var gset_bij.
+From iris.algebra Require Import gset gset_bij.
+From melocoton Require Import big_sepM_limited.
+From iris.proofmode Require Import proofmode.
+From melocoton.c_toy_lang Require Import lang melocoton.lang_instantiation melocoton.primitive_laws.
+From melocoton.ml_toy_lang Require Import lang melocoton.lang_instantiation melocoton.primitive_laws.
+From melocoton.interop Require Import linking_wp basics wrapper_wp wrapper_wp_block_sim.
+Import Wrap.
+
+
+Global Notation MLval := ML_lang.val.
+Global Notation Cval := C_lang.val.
+
+Definition forbidden_function_names : list string := ["alloc"; "registerroot"; "unregisterroot"; "modify"; "readfield"; "int2val"; "val2int"].
+
+
+Section Utils.
+
+Context {hlc : has_lc}.
+Context {Σ : gFunctors}.
+Context `{!heapGS_ML Σ, !heapGS_C Σ}.
+Context `{!invGS_gen hlc Σ}.
+Context `{!wrapperGS Σ}.
+
+Implicit Types P : iProp Σ.
+Import mlanguage.
+Notation mkPeC p T := ({| penv_prog := p; penv_proto := T |} : prog_environ _ Σ).
+Notation mkPeW p T := ({| weakestpre.penv_prog := p; weakestpre.penv_proto := T |} : weakestpre.prog_environ wrap_lang Σ).
+
+Notation spec := (string -d> list Cval -d> (Cval -d> iPropO Σ) -d> iPropO Σ).
+
+Definition WP_int2val_spec : spec := (λ n vl wp,
+   "(%θ & %z & HGC & -> & -> & HWP)" 
+    ∷ (∃ θ z, GC θ ∗ ⌜n = "int2val"⌝ ∗ ⌜vl = [C_lang.LitV $ C_lang.LitInt $ z]⌝ ∗ (∀ w, GC θ -∗ ⌜repr_lval θ (Lint z) w⌝ -∗ wp w )))%I.
+
+Definition WP_val2int_spec : spec := (λ n vl wp,
+   "(%θ & %w & %z & HGC & -> & %Hrepr & -> & HWP)" 
+    ∷ (∃ θ w z, GC θ ∗ ⌜n = "val2int"⌝ ∗ ⌜repr_lval θ (Lint z) w⌝ ∗ ⌜vl = [ w ]⌝ ∗ (GC θ -∗ wp (C_lang.LitV $ C_lang.LitInt $ z) )))%I.
+
+Definition WP_ext_call_spec : spec := (λ n vl wp,
+    WP_int2val_spec n vl wp ∨ WP_val2int_spec n vl wp)%I.
+
+Lemma WP_ext_call_sound s v T : WP_ext_call_spec s v T -∗ ⌜s ∈ forbidden_function_names⌝.
+Proof.
+  iIntros "[H|H]"; unfold WP_int2val_spec; unfold WP_val2int_spec; iNamed "H";
+  iPureIntro; unfold forbidden_function_names;
+  repeat (try done; try left; right).
+Qed.
+
+Notation wrap_return := (fun Φ (a:Cval) => (∃ θ' l v, GC θ' ∗ Φ v ∗ ⌜repr_lval θ' l a⌝ ∗ block_sim v l)%I).
+
+Section RootsRepr.
+
+(* We can decompose mem, the C heap, into a privmem, which is everything but the roots, and a memr, which are just the rooted cells *)
+Lemma make_repr θ roots_m mem : 
+    roots_are_live θ roots_m
+ -> map_Forall (λ k v, ∃ w , mem !! k = Some (Storing w) ∧ repr_lval θ v w) roots_m
+ -> ∃ privmem, repr θ roots_m privmem mem.
+Proof.
+  revert mem.
+  induction roots_m as [|l a roots_m Hin IH] using map_ind; intros mem Hlive Hforall.
+  + exists mem, ∅. split_and!.
+    * econstructor.
+    * eapply map_disjoint_empty_r.
+    * by rewrite map_empty_union.
+  + apply map_Forall_insert_1_1 in Hforall as Hforall2.
+    destruct Hforall2 as (w & Hw & Hrep).
+    specialize (IH (delete l mem)).
+    destruct IH as (privmem & memr & IH & Hdisj & Hunion).
+    1: intros l' g Hg; eapply Hlive; rewrite lookup_insert_ne; first done; intros ->; rewrite Hg in Hin; congruence.
+    1: apply map_Forall_lookup; intros i x Hinix;
+       eapply map_Forall_lookup_1 in Hforall.
+    1: destruct Hforall as (w' & H1 & H2); exists w'; repeat split; try done.
+    1: rewrite lookup_delete_ne; first done.
+    2: rewrite lookup_insert_ne; first done.
+    1-2: intros ->; rewrite Hin in Hinix; congruence.
+    assert (memr !! l = None) as HNone1.
+    1: apply not_elem_of_dom; erewrite <- repr_roots_dom; last done; by eapply not_elem_of_dom.
+    assert (privmem !! l = None) as Hnone2.
+    rewrite <- (lookup_union_r memr privmem); try done; rewrite <- Hunion; by apply lookup_delete.
+    eexists privmem, (<[l:=Storing w]> memr). split_and!.
+    * econstructor; try done; by eapply not_elem_of_dom.
+    * by apply map_disjoint_insert_r.
+    * erewrite <- insert_union_l. rewrite <- Hunion. rewrite insert_delete_insert.
+      apply map_eq_iff. intros i. destruct (decide (i = l)) as [-> |]; (try by rewrite lookup_insert); by rewrite lookup_insert_ne.
+Qed.
+
+Lemma set_to_none θ mem roots_m privmem :
+    repr θ roots_m privmem mem
+ -> gen_heap_interp mem
+ -∗ ([∗ map] a0↦v0 ∈ roots_m, ∃ w, a0 ↦C{DfracOwn 1} w ∗ ⌜repr_lval θ v0 w⌝)
+==∗ (gen_heap_interp (privmem ∪ ((λ _ : lval, None) <$> roots_m))
+    ∗[∗ set] a0 ∈ dom roots_m, a0 O↦ None).
+Proof.
+  intros (mm & Hrepr1 & Hrepr2 & Hrepr3).
+  induction Hrepr1 in Hrepr2,Hrepr3,mem,privmem|-*.
+  + iIntros "Hheap Hmap !>".
+    rewrite fmap_empty. rewrite dom_empty_L. rewrite map_union_empty.
+    rewrite map_empty_union in Hrepr3. subst mem. iFrame.
+    iApply big_sepS_empty. done.
+  + eapply not_elem_of_dom in H0,H1. iIntros "Hheap Hmap".
+    iPoseProof (big_sepM_insert) as "(Hb1 & _)"; first apply H0.
+    iPoseProof ("Hb1" with "Hmap") as "((%w' & Hw & %Hrepr4) & Hmap)".
+    pose proof (repr_lval_inj _ _ _ _ Hrepr4 H) as Heq; subst w'.
+    iMod (gen_heap_update with "Hheap Hw") as "(Hheap & Hw)".
+    specialize (IHHrepr1 (<[a:=None]> mem) (<[a:=None]> privmem)).
+    iMod (IHHrepr1 with "Hheap Hmap") as "(Hheap & Hmap)".
+    * eapply map_disjoint_insert_l_2; first done.
+      erewrite <- (delete_insert mem0); last done.
+      by eapply map_disjoint_delete_r.
+    * subst mem. erewrite <- insert_union_l.
+      rewrite insert_insert. by rewrite insert_union_r.
+    * iModIntro. iSplitL "Hheap".
+      - erewrite <- insert_union_l. rewrite insert_union_r.
+        2: eapply map_disjoint_Some_r; try done; by rewrite lookup_insert.
+        rewrite fmap_insert. iFrame.
+      - rewrite dom_insert_L. iApply big_sepS_insert; first by eapply not_elem_of_dom. iFrame.
+Qed.
+
+Lemma find_repr_lval_vv θ v : 
+   (forall γ, Lloc γ = v → γ ∈ dom θ)
+ → exists l, repr_lval θ v l.
+Proof.
+  intros H. destruct v as [z|a].
+  - eexists; by econstructor.
+  - destruct (θ !! a) as [va|] eqn:Heq.
+    2: eapply not_elem_of_dom in Heq; exfalso; apply Heq; apply H; done.
+    eexists; econstructor; apply Heq.
+Qed.
+
+Lemma find_repr_lval_vs θ vs : 
+   (forall γ, Lloc γ ∈ vs → γ ∈ dom θ)
+ → exists ls, Forall2 (repr_lval θ) vs ls.
+Proof.
+  intros H; induction vs as [|v vs IH] in H|-*.
+  - exists nil. econstructor.
+  - destruct IH as [ls IH]; first (intros γ Hγ; eapply H; right; done).
+    destruct (find_repr_lval_vv θ v) as [l Hl].
+    1: intros γ <-; apply H; by left.
+    eexists. econstructor; done.
+Qed.
+
+Lemma find_repr_roots θ roots privmem : 
+   roots_are_live θ roots
+ → dom privmem ## dom roots
+ → exists mem, repr θ roots privmem mem.
+Proof.
+  revert privmem. unfold repr.
+  induction roots as [|l a roots_m Hin IH] using map_ind; intros privmem Hlive Hdisj.
+  - exists privmem, ∅. split_and!.
+    + econstructor.
+    + eapply map_disjoint_empty_r.
+    + by rewrite map_empty_union.
+  - destruct (IH privmem) as (mem1 & memr1 & Hrepr1 & Hdisj1 & Heq1).
+    1: { intros a1 w1 H1; eapply Hlive; rewrite lookup_insert_ne; first done.
+         intros ->; rewrite Hin in H1; congruence. }
+    1: rewrite dom_insert_L in Hdisj; set_solver.
+    destruct (find_repr_lval_vv θ a) as (w & Hw).
+    1: intros γ <-; eapply Hlive; apply lookup_insert.
+    exists (<[l:=Storing w]> mem1), (<[l:=Storing w]> memr1). split_and!.
+    + econstructor. 1: done. 1:done. 2: erewrite <- repr_roots_dom; last apply Hrepr1. all: by eapply not_elem_of_dom.
+    + apply map_disjoint_dom in Hdisj1. apply map_disjoint_dom.
+      rewrite dom_insert_L. rewrite dom_insert_L in Hdisj. set_solver.
+    + erewrite Heq1. now rewrite insert_union_l.
+Qed.
+
+
+Lemma set_to_some θ mem roots_m privmem :
+    repr θ roots_m privmem mem
+ -> gen_heap_interp (privmem ∪ ((λ _ : lval, None) <$> roots_m))
+ -∗ ([∗ set] a ∈ dom roots_m, a O↦ None)
+ ==∗ gen_heap_interp mem
+     ∗ ([∗ map] a↦v ∈ roots_m, ∃ w, a ↦C{DfracOwn 1} w ∗ ⌜repr_lval θ v w⌝).
+Proof.
+  intros (mm & Hrepr1 & Hrepr2 & Hrepr3).
+  induction Hrepr1 in Hrepr2,Hrepr3,mem,privmem|-*.
+  + iIntros "Hheap Hset !>".
+    rewrite fmap_empty. rewrite dom_empty_L. rewrite map_union_empty.
+    rewrite map_empty_union in Hrepr3. subst mem. iFrame.
+    iApply big_sepM_empty. done.
+  + eapply not_elem_of_dom in H0,H1. iIntros "Hheap Hset".
+    rewrite dom_insert_L.
+    iPoseProof (big_sepS_insert) as "(Hb1 & _)"; first eapply not_elem_of_dom_2, H0.
+    iPoseProof ("Hb1" with "Hset") as "(Hw & Hset)".
+    rewrite fmap_insert. rewrite <- insert_union_r.
+    2: eapply map_disjoint_Some_r; first done; by rewrite lookup_insert.
+    iMod (gen_heap_update _ _ _ (Storing w) with "Hheap Hw") as "(Hheap & Hw)".
+    rewrite insert_insert.
+    rewrite insert_union_l.
+    iMod (IHHrepr1 with "Hheap Hset") as "(Hheap & Hset)".
+    * eapply map_disjoint_insert_l_2; first done.
+      erewrite <- (delete_insert mem0); last done.
+      by eapply map_disjoint_delete_r.
+    * done.
+    * rewrite <- insert_union_r; last done.
+      subst mem. rewrite insert_union_l. iModIntro.
+      iFrame.
+      iApply (big_sepM_insert_2 with "[Hw] Hset").
+      iExists w. iFrame. done.
+Qed.
+
+End RootsRepr.
+
+Section ChiZetaConstruction.
+
+Definition lookup_reversed (χ : lloc_map) ℓ := {γ | χ !! γ = Some (LlocPublic ℓ)}.
+
+Definition find_in_χ (χ:lloc_map) ℓ : sum (lookup_reversed χ ℓ) (lookup_reversed χ ℓ -> False).
+Proof.
+  pose (map_to_set (fun γ ll => match ll with LlocPrivate => None | LlocPublic ℓ' => if decide (ℓ' = ℓ) then Some γ else None end) χ : gset _) as Hset.
+  epose (filter (fun k => is_Some (k)) Hset) as Hset2.
+  destruct (elements Hset2) as [|[γ|] ?] eqn:Heq.
+  - right. intros (γ & Hγ).
+    apply elements_empty_inv in Heq. apply gset_leibniz in Heq.
+    eapply filter_empty_not_elem_of_L. 2: apply Heq. 1: apply _.
+    2: eapply elem_of_map_to_set.
+    2: exists γ, (LlocPublic ℓ); split; done.
+    rewrite decide_True; done. Unshelve. all: apply _.
+  - left. exists γ.
+    assert (Some γ ∈ Hset2).
+    1: eapply elem_of_elements; rewrite Heq; left.
+    eapply elem_of_filter in H. destruct H as [_ H].
+    eapply elem_of_map_to_set in H.
+    destruct H as (i & ll & H1 & H2).
+    destruct ll; try congruence.
+    destruct decide; try congruence.
+  - exfalso. assert (None ∈ Hset2).
+    + eapply elem_of_elements. rewrite Heq. left.
+    + apply elem_of_filter in H. destruct H as [[? Hc]?]. congruence.
+Defined.
+
+Lemma ensure_in_χ_pub χ ℓ : lloc_map_inj χ → exists χ' γ, lloc_map_mono χ χ' ∧ χ' !! γ = Some (LlocPublic ℓ) ∧ ∀ γ' r, γ' ≠ γ → χ' !! γ' = r → χ !! γ' = r.
+Proof.
+  intros Hinj.
+  destruct (find_in_χ χ ℓ) as [[γ Hgam]|Hnot].
+  1: exists χ, γ; done.
+  eexists (<[fresh (dom χ) := LlocPublic ℓ]> χ), _.
+  erewrite lookup_insert; split_and!. 2: done.
+  2: intros γ' r Hne H1; by rewrite lookup_insert_ne in H1.
+  split.
+  1: eapply insert_subseteq, not_elem_of_dom, is_fresh.
+  intros γ1 γ2 ℓ' [[? ?]|[? ?]]%lookup_insert_Some [[? ?]|[? ?]]%lookup_insert_Some; subst.
+  1: done.
+  3: by eapply Hinj.
+  all: exfalso; eapply Hnot; eexists _; erewrite H0, H2; done.
+Qed.
+
+Definition extended_to (χold : lloc_map) (ζ : lstore) (χnew : lloc_map) :=
+  lloc_map_mono χold χnew ∧ dom χold ## dom ζ ∧ is_private_blocks χnew ζ.
+
+Lemma extended_to_inj χ1 ζ χ2 : extended_to χ1 ζ χ2 → lloc_map_inj χ2.
+Proof.
+  intros (H&_); apply H.
+Qed.
+
+Lemma extended_to_dom_subset χ1 ζ χ2 : extended_to χ1 ζ χ2 → dom ζ ⊆ dom χ2.
+Proof.
+  intros (H1&H2&H3).
+  eapply elem_of_subseteq. intros γ Hx; eapply elem_of_dom_2. by apply H3.
+Qed.
+
+Definition allocate_in_χ_priv (χold : lloc_map) v : lloc_map_inj χold → exists χnew γ, extended_to χold {[γ := v]} χnew.
+Proof.
+  intros Hinj.
+  eexists (<[fresh (dom χold) := LlocPrivate]> χold), (fresh (dom χold)).
+  unfold extended_to; split_and!; first split.
+  - eapply insert_subseteq, not_elem_of_dom, is_fresh.
+  - intros γ1 γ2 ℓ' [[? ?]|[? ?]]%lookup_insert_Some [[? ?]|[? ?]]%lookup_insert_Some; subst; try congruence.
+    by eapply Hinj.
+  - rewrite dom_singleton_L. eapply disjoint_singleton_r. by apply is_fresh.
+  - intros x. rewrite dom_singleton_L. intros ->%elem_of_singleton.
+    eapply lookup_insert.
+Qed.
+
+Lemma disjoint_weaken T `{Countable T} (A1 A2 B1 B2 : gset T) : A1 ## B1 → A2 ⊆ A1 → B2 ⊆ B1 → A2 ## B2.
+Proof.
+  intros HD H1 H2.
+  apply elem_of_disjoint.
+  intros x HA HB.
+  edestruct (@elem_of_disjoint) as [HL _]; eapply HL.
+  - apply HD.
+  - eapply elem_of_weaken; first apply HA. done.
+  - eapply elem_of_weaken; first apply HB. done.
+Qed.
+
+Lemma extended_to_trans (χ1 χ2 χ3 : lloc_map) (ζ1 ζ2 : lstore) : 
+  extended_to χ1 ζ1 χ2 →
+  extended_to χ2 ζ2 χ3 →
+  extended_to χ1 (ζ1 ∪ ζ2) χ3 /\ ζ1 ##ₘ ζ2.
+Proof.
+  intros (HA1 & HA2 & HA3) (HB1 & HB2 & HB3). unfold extended_to; split_and!.
+  - split; last apply HB1. etransitivity; first apply HA1; apply HB1.
+  - erewrite dom_union_L. eapply disjoint_union_r. split; first done.
+    eapply disjoint_weaken. 1: apply HB2. 2: done. apply subseteq_dom, HA1.
+  - intros γ. rewrite dom_union_L. intros [H|H]%elem_of_union; last by apply HB3.
+    eapply lookup_weaken; first by apply HA3.
+    apply HB1.
+  - eapply map_disjoint_dom. eapply disjoint_weaken. 1: apply HB2. 2: done.
+    eapply extended_to_dom_subset; done.
+Qed.
+
+Lemma extended_to_trans_2 (χ1 χ2 χ3 : lloc_map) (ζ1 ζ2 : lstore) : 
+  extended_to χ1 ζ1 χ2 →
+  extended_to χ2 ζ2 χ3 →
+  extended_to χ1 (ζ2 ∪ ζ1) χ3 /\ ζ1 ##ₘ ζ2.
+Proof.
+  intros H1 H2.
+  destruct (extended_to_trans χ1 χ2 χ3 ζ1 ζ2) as (H3&H4). 1-2: done.
+  erewrite map_union_comm; done.
+Qed.
+
+Lemma extended_to_refl χ1 :
+  lloc_map_inj χ1 →
+  extended_to χ1 ∅ χ1.
+Proof.
+  by repeat split.
+Qed.
+
+Lemma extended_to_mono χ1 χ2 :
+  lloc_map_mono χ1 χ2 →
+  extended_to χ1 ∅ χ2.
+Proof.
+  intros (H1 & H2); by repeat split.
+Qed.
+
+Lemma is_val_extended_to_weaken χ1 χ2 ζ1 ζ2 v lv:
+  is_val χ1 ζ1 v lv →
+  extended_to χ1 ζ2 χ2 →
+  is_val χ2 (ζ1 ∪ ζ2) v lv.
+Proof.
+  intros H1 (H21&H22&H23).
+  eapply is_val_mono; last done.
+  1: apply H21.
+  apply map_union_subseteq_l.
+Qed.
+
+Lemma deserialize_ML_value χMLold v :  
+  lloc_map_inj χMLold
+→ ∃ χC ζimm lv,
+    extended_to χMLold ζimm χC
+  ∧ is_val χC ζimm v lv.
+Proof.
+  induction v as [[x|bo| |ℓ]| |v1 IHv1 v2 IHv2|v IHv|v IHv] in χMLold|-*; intros Hinj.
+  1-3,5: eexists χMLold, ∅, _; split_and!; [by eapply extended_to_refl | econstructor ].
+  Unshelve. 5: exact (Lloc 0). (* what happens for functions *)
+  - destruct (ensure_in_χ_pub χMLold ℓ) as (χ' & γ & Hχ' & Hγ & _); first done.
+    exists χ', ∅, (Lloc γ); (split_and!; last by econstructor).
+    by eapply extended_to_mono.
+  - destruct (IHv1 χMLold) as (χ1 & ζ1 & lv1 & Hext1 & Hlv1); first done.
+    destruct (IHv2 χ1) as (χ2 & ζ2 & lv2 & Hext2 & Hlv2); first by eapply extended_to_inj.
+    pose (Immut,(TagDefault,[lv1;lv2])) as blk.
+    edestruct (allocate_in_χ_priv χ2 blk) as (χ3 & γ & Hext3); first by eapply extended_to_inj.
+    eassert (extended_to χMLold _ χ3).
+    1: do 2 (eapply extended_to_trans; last done); done.
+    do 3 eexists; split; first done.
+    econstructor.
+    + rewrite lookup_union_r; first by erewrite lookup_singleton.
+      eapply map_disjoint_Some_r. 1: eapply extended_to_trans_2; first eapply extended_to_trans; done.
+      apply lookup_singleton.
+    + eapply is_val_extended_to_weaken; last done.
+      eapply is_val_extended_to_weaken; done.
+    + eapply is_val_extended_to_weaken; last done.
+      eapply is_val_mono; last done; try done.
+      eapply map_union_subseteq_r. eapply extended_to_trans; done.
+  - destruct (IHv χMLold) as (χ1 & ζ1 & lv1 & Hext1 & Hlv1); first done.
+    epose (Immut,(_,[lv1])) as blk.
+    edestruct (allocate_in_χ_priv χ1 blk) as (χ3 & γ & Hext3); first by eapply extended_to_inj.
+    eassert (extended_to χMLold _ χ3).
+    1: (eapply extended_to_trans; last done); done.
+    do 3 eexists; split; first done.
+    econstructor.
+    + rewrite lookup_union_r; first by erewrite lookup_singleton.
+      eapply map_disjoint_Some_r. 1: eapply extended_to_trans_2; done.
+      apply lookup_singleton.
+    + eapply is_val_extended_to_weaken; done.
+  - destruct (IHv χMLold) as (χ1 & ζ1 & lv1 & Hext1 & Hlv1); first done.
+    epose (Immut,(_,[lv1])) as blk.
+    edestruct (allocate_in_χ_priv χ1 blk) as (χ3 & γ & Hext3); first by eapply extended_to_inj.
+    eassert (extended_to χMLold _ χ3).
+    1: (eapply extended_to_trans; last done); done.
+    do 3 eexists; split; first done.
+    econstructor.
+    + rewrite lookup_union_r; first by erewrite lookup_singleton.
+      eapply map_disjoint_Some_r. 1: eapply extended_to_trans_2; done.
+      apply lookup_singleton.
+    + eapply is_val_extended_to_weaken; done.
+Qed.
+
+Lemma deserialize_ML_values χMLold vs :  
+  lloc_map_inj χMLold
+→ ∃ χC ζimm lvs,
+    extended_to χMLold ζimm χC
+  ∧ Forall2 (is_val χC ζimm) vs lvs.
+Proof.
+  induction vs as [|v vs IH] in χMLold|-*; intros Hinj.
+  - eexists χMLold, ∅, _; split_and!; [by eapply extended_to_refl | econstructor ].
+  - destruct (deserialize_ML_value χMLold v Hinj) as (χ1 & ζ1 & lv & Hext1 & Hlv1).
+    destruct (IH χ1) as (χ2 & ζ2 & lvs & Hext2 & Hlv2); first by eapply extended_to_inj.
+    eassert (extended_to χMLold _ χ2) by by eapply extended_to_trans.
+    eexists _, _, (lv::lvs). split_and!; first done.
+    econstructor.
+    + by eapply is_val_extended_to_weaken.
+    + eapply Forall2_impl; first done.
+      intros v' lv' H1. eapply is_val_mono; last done; try done.
+      eapply map_union_subseteq_r, extended_to_trans; done.
+Qed.
+
+Lemma deserialize_ML_block χMLold vs :  
+  lloc_map_inj χMLold
+→ ∃ χC ζimm blk,
+    extended_to χMLold ζimm χC
+  ∧ is_heap_elt χC ζimm vs blk.
+Proof.
+  intros H.
+  destruct (deserialize_ML_values χMLold vs H) as (χC & ζimm & lvs & H1 & H2).
+  by exists χC, ζimm, (Mut,(TagDefault,lvs)).
+Qed.
+
+
+Lemma is_store_blocks_mono_weaken χ1 χ2 ζ σ:
+  is_store_blocks χ1 ζ σ →
+  lloc_map_mono χ1 χ2 →
+  is_store_blocks χ2 ζ σ.
+Proof.
+  intros (H1&H2) [Hsub H3]. split.
+  - intros x Hx. destruct (H1 x Hx) as [y Hy]; exists y.
+    eapply lookup_weaken; done.
+  - intros γ; destruct (H2 γ) as [H2L H2R]; split.
+    + intros H; destruct (H2L H) as (ℓ&Vs&HH1&HH2). do 2 eexists; repeat split; try done.
+      eapply lookup_weaken; done.
+    + intros (ℓ&Vs&HH1&HH2).
+      apply H2R. do 2 eexists; repeat split; try done.
+      destruct (H1 ℓ) as (γ2&Hγ2); first by eapply elem_of_dom_2.
+      rewrite <- Hγ2.
+      eapply lookup_weaken in Hγ2; last done.
+      f_equiv. eapply H3; done.
+Qed.
+
+Lemma is_heap_elt_weaken χ ζ vs blk ζ' χ' :
+  is_heap_elt χ ζ vs blk
+→ χ ⊆ χ'
+→ ζ ⊆ ζ'
+→ is_heap_elt χ' ζ' vs blk.
+Proof.
+  intros H1 H2 H3.
+  inversion H1; subst.
+  econstructor. eapply Forall2_impl; first done.
+  intros x y H4; eapply is_val_mono; last done. all:done.
+Qed.
+
+Lemma is_heap_elt_weaken_2 χ ζ vs blk ζ' χ' :
+  is_heap_elt χ ζ vs blk
+→ extended_to χ' ζ χ
+→ dom ζ' ⊆ dom χ'
+→ is_heap_elt χ (ζ' ∪ ζ) vs blk.
+Proof.
+  intros H1 H2 H3.
+  eapply is_heap_elt_weaken. 1: done.
+  1: done. eapply map_union_subseteq_r.
+  eapply map_disjoint_dom. eapply disjoint_weaken.
+  1: apply H2. 1-2:done.
+Qed.
+
+Lemma deserialize_ML_heap χMLold σ : 
+  lloc_map_inj χMLold
+→ ∃ χC ζσ ζnewimm,
+    extended_to χMLold ζnewimm χC
+  ∧ is_store_blocks χC σ ζσ
+  ∧ is_store χC (ζσ ∪ ζnewimm) σ.
+Proof.
+  revert χMLold.
+  induction σ as [|ℓ [vv|] σ Hin IH] using map_ind; intros χMLold HχMLold .
+  - exists χMLold, ∅, ∅; split_and!. 2: econstructor.
+    + by eapply extended_to_refl.
+    + intros γ; rewrite dom_empty_L; done.
+    + split; rewrite dom_empty_L. 1: done.
+      intros (ℓ & Vs & H1 & H2). exfalso. rewrite lookup_empty in H2. done.
+    + intros ℓ Vs γ blk Hc. exfalso. rewrite lookup_empty in Hc. done.
+  - destruct (IH χMLold) as (χ0 & ζσ & ζi0 & Hext & Hstbl & Hstore). 1: done.
+    destruct (ensure_in_χ_pub χ0 ℓ) as (χ1 & γ & Hχ1 & Hγ & Hold); first by eapply extended_to_inj.
+    apply extended_to_mono in Hχ1.
+    destruct (deserialize_ML_block χ1 vv) as (χ2 & ζi2 & lvs & Hext2 & Helt); first by eapply extended_to_inj.
+    edestruct (extended_to_trans) as (HextA&Hdisj1). 1: exact Hext. 1: eapply extended_to_trans; done.
+    rewrite map_empty_union in Hdisj1.
+    rewrite map_empty_union in HextA.
+    assert (is_store_blocks χ2 (<[ℓ:=Some vv]> σ) (<[γ:=lvs]> ζσ)) as Hstore2.
+    1: {eapply is_store_blocks_restore_loc.
+        * eapply is_store_blocks_mono_weaken; first done. eapply extended_to_trans; done.
+        * apply Hext2.
+        * eapply lookup_weaken. 1: done. apply Hext2.
+        * by right. }
+    assert (dom (<[γ:=lvs]> ζσ ∪ ζi0) ⊆ dom χ1) as Hsub3.
+    { rewrite dom_union_L. eapply union_subseteq. split.
+      * rewrite dom_insert_L. apply union_subseteq. split.
+        eapply singleton_subseteq_l; first by eapply elem_of_dom_2.
+        eapply elem_of_subseteq; intros k Hk.
+        destruct Hstbl as (HH1&HH2). apply HH2 in Hk. destruct Hk as (?&?&H1&H2).
+        eapply elem_of_dom_2. eapply lookup_weaken; first apply H1.
+        eapply Hχ1.
+      * etransitivity; last eapply subseteq_dom, Hχ1.
+        eapply extended_to_dom_subset; done. }
+    eexists χ2, (<[γ := lvs]> ζσ), (ζi0 ∪ ζi2). split_and!. 1-2:done.
+    intros ℓ' vs γ' blk H1 H2 H3.  destruct HextA as (HH1&HH2&HH3).
+    apply lookup_union_Some in H3. 1: destruct H3 as [H3|H3].
+    3: { eapply map_disjoint_dom; eapply elem_of_disjoint.
+         intros x Hx1 Hx2; specialize (HH3 x Hx2). destruct Hstore2 as [HHL HHR].
+         apply HHR in Hx1. destruct Hx1 as (l1 & Vs1 & ? & ?); congruence. }
+    2: { rewrite HH3 in H2; last by eapply elem_of_dom_2. congruence. }
+    apply lookup_insert_Some in H3. destruct H3 as [[? ?]|[Hne H3]].
+    + subst. rewrite map_union_assoc.
+      eapply lookup_weaken in Hγ. 2: eapply Hext2. rewrite Hγ in H2. injection H2; intros ->.
+      rewrite lookup_insert in H1. injection H1; intros ->.
+      by eapply is_heap_elt_weaken_2.
+    + eapply lookup_insert_Some in H1. destruct H1 as [[-> H]|[Hne1 H1]].
+      1: {exfalso. apply Hne. eapply HH1. 2: done. eapply lookup_weaken; first done. apply Hext2. }
+      assert (χ0 !! γ' = Some (LlocPublic ℓ')) as H2'.
+      1: {destruct Hstbl as [HHL HHR]. destruct (HHL ℓ') as (gg&Hgg); first by eapply elem_of_dom_2.
+          rewrite <- Hgg; f_equal. eapply HH1. 1: done. eapply lookup_weaken; first done. etransitivity; last eapply Hext2; eapply Hχ1. }
+      eapply is_heap_elt_weaken.
+      1: eapply Hstore. 1: done. 3: etransitivity; first eapply Hχ1; last apply Hext2.
+      2: erewrite lookup_union_l; first done. 1: done.
+      1: eapply not_elem_of_dom; intros H; eapply Hext in H; congruence.
+      etransitivity; first eapply map_union_mono_l.
+      2: etransitivity; first eapply map_union_mono_r. 4: done.
+      1: eapply map_union_subseteq_l.
+      1: eapply is_store_blocks_is_private_blocks_disjoint; done.
+      eapply insert_subseteq, not_elem_of_dom.
+      intros H. destruct Hstbl as [HHL HHR]. eapply HHR in H.
+      destruct H as (?&?&Heq1&HeqF). eapply lookup_weaken in Heq1; first erewrite Hγ in Heq1. 2: apply Hχ1.
+      injection Heq1; intros ->; rewrite HeqF in Hin; congruence.
+  - destruct (IH χMLold) as (χ0 & ζσ & ζi0 & Hext & Hstbl & Hstore). 1: done.
+    destruct (ensure_in_χ_pub χ0 ℓ) as (χ1 & γ & Hχ1 & Hγ & Hold); first by eapply extended_to_inj.
+    edestruct (extended_to_trans) as (HextA&Hdisj1); first exact Hext. 1: eapply extended_to_mono, Hχ1.
+    exists χ1, ζσ, ζi0. split_and!. 2: destruct Hstbl as [HL HR]; split.
+    + rewrite map_union_empty in HextA. done.
+    + rewrite dom_insert_L. intros ℓ0 [->%elem_of_singleton|H]%elem_of_union.
+      1: eexists; done.
+      destruct (HL ℓ0 H) as (γ1&Hγ1). exists γ1; eapply lookup_weaken; first done.
+      eapply Hχ1.
+    + intros γ0; specialize (HR γ0) as (HRL&HRR). split.
+      1: intros H; destruct (HRL H) as (ℓ0 & Vs & H3 & H5); do 2 eexists;
+        split; first (eapply lookup_weaken; first done; eapply Hχ1);
+        rewrite lookup_insert_ne; first done;
+        intros ->; rewrite Hin in H5; congruence.
+      intros (ℓ0&Vs&HH1&HH2).
+      rewrite lookup_insert_Some in HH2; destruct HH2 as [[? ?]|[Hne HH2]].
+      1: congruence.
+      eapply HRR. eexists ℓ0, Vs. split; last done.
+      eapply elem_of_dom_2 in HH2.
+      destruct (HL ℓ0 HH2) as (γ1&Hγ1). rewrite <- Hγ1. f_equal.
+      eapply Hχ1; try done. eapply lookup_weaken, Hχ1; done.
+    + intros ℓ1 vs γ1 blk [[? ?]|[? H1]]%lookup_insert_Some H2 H3; try congruence.
+      eapply is_heap_elt_weaken. 1: eapply Hstore; try done.
+      3: done. 2: eapply Hχ1.
+      destruct Hstbl as [HHL HHR].
+      destruct (HHL ℓ1) as (k1&Hk1); first by eapply elem_of_dom_2.
+      rewrite <- Hk1. f_equal. eapply Hχ1; try done. eapply lookup_weaken, Hχ1; done.
+Qed.
+
+Lemma deserialize_ML_heap_extra ζMLold χMLold σ : 
+  lloc_map_inj χMLold
+→ dom ζMLold ⊆ dom χMLold
+→ (map_Forall (fun _ ℓ => σ !! ℓ = Some None) (pub_locs_in_lstore χMLold ζMLold))
+→ ∃ χC ζσ ζnewimm,
+    extended_to χMLold ζnewimm χC
+  ∧ is_store_blocks χC σ ζσ
+  ∧ ζMLold ##ₘ (ζσ ∪ ζnewimm)
+  ∧ is_store χC (ζMLold ∪ ζσ ∪ ζnewimm) σ.
+Proof.
+  intros H1 H2 H3.
+  destruct (deserialize_ML_heap χMLold σ) as (χC&ζσ&ζi&HA1&HA2&HA3). 1: apply H1.
+  assert (ζMLold ##ₘ ζσ ∪ ζi) as Hdisj.
+  1: eapply map_disjoint_union_r; split; last (eapply map_disjoint_dom, disjoint_weaken; first apply HA1; done).
+  1: { eapply map_disjoint_spec. intros γ b1 b2 HH1 HH2.
+       destruct HA2 as [_ HA2R]. eapply elem_of_dom_2 in HH2. apply HA2R in HH2.
+       destruct HH2 as (ℓ & Vs & HH7 & HH8).
+       erewrite (map_Forall_lookup_1 _ _ _ _ H3) in HH8.
+       2: { eapply elem_of_dom_2 in HH1. erewrite pub_locs_in_lstore_lookup; first done; first done.
+            eapply elem_of_weaken in H2; last done.
+            eapply elem_of_dom in H2; destruct H2 as [k Hk]. rewrite Hk. 
+            eapply lookup_weaken in Hk; first erewrite HH7 in Hk. 2: eapply HA1. done. }
+       congruence. }
+  do 3 eexists; split_and!; try done.
+  - intros ℓ vs γ b He1 He2 He3.
+    eapply is_heap_elt_weaken. 1: eapply HA3; try done. 2: done.
+    + rewrite <- map_union_assoc in He3. eapply lookup_union_Some in He3; destruct He3; try done.
+      destruct (HA2) as [HL HR]. destruct (HR γ) as [HRL HRR]. eapply elem_of_dom in HRR. destruct HRR as [vv Hvv].
+      2: do 2 eexists; done.
+      exfalso. erewrite map_disjoint_Some_r in H; try congruence. 1: done.
+      erewrite lookup_union_Some_l; last done; first done.
+    + erewrite <- map_union_assoc. eapply map_union_subseteq_r. done.
+Qed.
+
+End ChiZetaConstruction.
+
+Section ThetaConstruction.
+
+Lemma collect_dom_θ_vs (θdom : gset lloc) (vs : list lval) : exists θdom' : gset lloc, forall γ, (Lloc γ ∈ vs ∨ γ ∈ θdom) ↔ γ ∈ θdom'.
+Proof.
+  induction vs as [|[|ℓ] vs (θdom1 & IH)].
+  - exists θdom. intros γ. split; last eauto. intros [[]%not_elem_of_nil|?]; done.
+  - exists θdom1. intros γ. split.
+    + intros [[Hc|H]%elem_of_cons|?]; try congruence; apply IH. 1: by left. by right.
+    + intros [H|H]%IH; last by right. left. right. done.
+  - exists (θdom1 ∪ {[ ℓ ]}). intros γ. split.
+    + intros [[Hc|H]%elem_of_cons|?]; eapply elem_of_union. 1: right; eapply elem_of_singleton; congruence.
+      all: left; apply IH. 1: by left. by right.
+    + intros [[H|H]%IH| ->%elem_of_singleton]%elem_of_union. 1: left; right; done. 1: right; done.    
+      left; left; done.
+Qed.
+
+Lemma collect_dom_θ_ζ_blocks (θdom : gset lloc) (ζ : lstore) : exists θdom' : gset lloc,
+    forall γ, ((exists γ1 m t vs, ζ !! γ1 = Some (m, (t, vs)) ∧ Lloc γ ∈ vs) ∨ γ ∈ θdom) ↔ γ ∈ θdom'.
+Proof.
+  induction ζ as [|k [m [t vs]] ζ Hne (θdom1 & Hdom1)] using map_ind.
+  - exists θdom; split.
+    + intros [(γ1&m&t&vs&H1&H2)|Hold]; last done.
+      rewrite lookup_empty in H1; done.
+    + intros H; by right.
+  - destruct (collect_dom_θ_vs θdom1 vs) as (θdom2 & Hdom2).
+    exists θdom2. intros γ; split.
+    + intros [(γ1&m'&t'&vs'&[[-> Hinj]|[Hne2 Hin]]%lookup_insert_Some&H2)|Hold].
+      1: apply Hdom2; left; congruence.
+      1: apply Hdom2; right; apply Hdom1; left; by repeat eexists.
+      1: apply Hdom2; right; apply Hdom1; right; done.
+    + intros [H|[(γ1&m'&t'&vs'&H1&H2)|H]%Hdom1]%Hdom2.
+      1: left; do 4 eexists; split; first eapply lookup_insert; done.
+      2: by right.
+      left; do 4 eexists; split; last done; first rewrite lookup_insert_ne; first done.
+      intros ->; rewrite Hne in H1; congruence.
+Qed.
+
+Lemma collect_dom_θ_ζ (θdom : gset lloc) (ζ : lstore) : exists θdom' : gset lloc,
+    forall γ, (γ ∈ dom ζ ∨ (exists γ1 m t vs, ζ !! γ1 = Some (m, (t, vs)) ∧ Lloc γ ∈ vs) ∨ γ ∈ θdom) ↔ γ ∈ θdom'.
+Proof.
+  destruct (collect_dom_θ_ζ_blocks θdom ζ) as (θdom1 & Hdom1).
+  exists (dom ζ ∪ θdom1). intros γ; split.
+  - (intros [H|H]; apply elem_of_union); first by left.
+    right; apply Hdom1; done.
+  - intros [H|H]%elem_of_union; first by left. right; by apply Hdom1.
+Qed.
+
+Lemma collect_dom_θ_roots (θdom : gset lloc) (roots : roots_map) : exists θdom' : gset lloc,
+    forall γ, ((exists k, roots !! k = Some (Lloc γ)) ∨ γ ∈ θdom) ↔ γ ∈ θdom'.
+Proof.
+  induction roots as [|k [z|l] roots Hne (θdom1 & IH)] using map_ind.
+  - exists θdom. intros γ. split; last eauto. intros [[? H%lookup_empty_Some]|?]; done.
+  - exists θdom1. intros γ. split.
+    + intros [[k1 [[-> ?]|[H1 H2]]%lookup_insert_Some]|?]; try congruence; apply IH. 2: by right. left. by eexists.
+    + intros [[k' Hk]|H]%IH; last by right. left. exists k'. rewrite lookup_insert_ne; first done. intros ->; rewrite Hne in Hk; done.
+  - exists (θdom1 ∪ {[ l ]}). intros γ. split.
+    + intros [[k1 [[-> ?]|[H1 H2]]%lookup_insert_Some]|?]; try congruence; eapply elem_of_union. 1: right; eapply elem_of_singleton; congruence.
+      all: left; apply IH. 2: by right. left; by eexists.
+    + intros [[[k' Hk]|H]%IH| ->%elem_of_singleton]%elem_of_union. 2: by right. 2: left; exists k; by rewrite lookup_insert.
+      left; exists k'; rewrite lookup_insert_ne; first done. intros ->; rewrite Hne in Hk; congruence.
+Qed.
+
+Lemma injectivify_map (S : gset lloc) : exists M : addr_map, dom M = S ∧ gmap_inj M.
+Proof.
+  induction S as [|s S Hne (M & <- & Hinj)] using set_ind_L.
+  - exists ∅; split; first by rewrite dom_empty_L. intros ??? H1; exfalso. rewrite lookup_empty in H1; done.
+  - exists (<[s := fresh (codom M)]> M). split.
+    1: by rewrite dom_insert_L.
+    apply gmap_inj_extend; try done.
+    intros k' v' H%codom_spec_2 <-. unshelve eapply is_fresh; last exact H. all: apply _.
+Qed.
+
+End ThetaConstruction.
+
+Section CallFacts.
+
+
+Implicit Type (p : language.prog C_lang).
+
+Notation fillCCall K s vv := (language.fill K (language.of_class C_lang (ExprCall s vv))).
+
+Lemma call_no_StepCS vv p s K mem ec' mem' T :
+  p !! s = None →
+  ~ (language.language.prim_step p (fillCCall K s vv) mem ec' mem' T).
+Proof.
+  intros Hno H4.
+  eapply prim_step_inv in H4.
+  destruct H4 as (K' & e1' & e2' & Heq1 & Heq2 & Hhead).
+  subst ec'. symmetry in Heq1. epose proof Heq1 as Heq2.
+  eapply (language.call_in_ctx K' K e1' s vv) in Heq1 as [(K'' & ->)|(v & <-)].
+  2: eapply language.val_head_step, Hhead.
+  rewrite <- language.fill_comp in Heq2.
+  eapply language.fill_inj in Heq2. subst e1'. epose proof Hhead as Hhead2.
+  eapply language.head_ctx_step_val in Hhead as [H|[x H]]. 2: apply language.language.of_to_val in H; cbn in H; done.
+  subst K''. rewrite language.fill_empty in Hhead2.
+  eapply (language.call_head_step p s vv) in Hhead2 as (fn & Hne & _).
+  cbn in Hno. rewrite Hno in Hne. congruence.
+Qed.
+
+
+Lemma call_no_RetS vv p s K r :
+  p !! s = None →
+  ~ (C_lang.to_val (fillCCall K s vv) = Some r).
+Proof.
+  intros Hno H4%C_lang.of_to_val.
+  edestruct (language.fill_class K) as [-> | [v Hv]].
+  - exists (ExprVal r); erewrite <- H4; done.
+  - cbn in H4. congruence.
+  - unfold language.language.to_val in Hv. by rewrite language.to_of_class in Hv.
+Qed.
+
+Lemma call_inversion vv p s K K' ec s' vv' :
+  p !! s = None →
+  language.fill K' ec = fillCCall K s vv →
+  language.to_call ec = Some (s', vv')
+  → s' = s ∧ vv' = vv ∧ K' = K.
+Proof.
+  intros H1 H2 H3. epose proof H2 as H2'.
+  eapply language.call_in_ctx in H2' as [(K'' & ->)|(v & Hv)].
+  - rewrite <- language.fill_comp in H2. apply language.fill_inj in H2.
+    subst ec. unfold language.to_call in H3.
+    edestruct (language.to_class) as [[|]|] eqn:Heq; try congruence.
+    edestruct (language.fill_class' K'') as [->|[v Hv]]; first by eexists.
+    2: rewrite language.to_of_class in Hv; done.
+    cbn in Heq. rewrite c_toy_lang.melocoton.lang_instantiation.map_unmap_val in Heq.
+    split_and!; cbn; congruence.
+  - subst ec. cbn in H3. done.
+Qed.
+
+End CallFacts.
+
+End Utils.
+
+
+Global Ltac inversion_call_step Hstep ww :=
+      let Heq1 := fresh "Heq1" in let Heq2 := fresh "Heq2" in
+      inversion Hstep;
+        first (exfalso; by eapply (call_no_StepCS ww));
+        first (exfalso; by eapply (call_no_RetS ww));
+        (edestruct (call_inversion ww) as (Heq1&Heq2&<-); first done; first done; first done; try (exfalso; congruence));
+        ((try injection Heq1); (try injection Heq2); repeat (first [intros -> | intros <-])).
+
+
